## Theorem: Let \( f, g: \mathbb{R} \rightarrow \mathbb{R} \) be differentiable functions such that

- \( f(0)=g(0) \),
- \( f^{\prime}(x) \leq g^{\prime}(x) \) for all \( x \geq 0 \).

Show that \( f(x) < q(x) \) for all \( x \geq 0 \).


## Proof: * Show that $f'(x)\leq g'(x)$ for all $x\geq 0$. 

Let $h:\mathbb{R} \longrightarrow \mathbb{R}$ be a function s.t. $h(x)=g(x)-f(x)$
$\forall x \in \mathbb{R}$.

from algebra of differentiable functions, $h$ is diff. on $\mathbb{R}$ (as $g$, $f$ are diff. on $\mathbb{R}$) and $h'(x)=g'(x)-f'(x)$
$\forall x \in \mathbb{R}$. 

we have $h(x)=g(x)-f(x)=0$ (as $g(0)=f(0)$
is given).

Let $x>0$. Since $h$ is diff. on $\mathbb{R}$, it is differentiable on $[-1,x] = [0,x]$  ($x+1>0 \implies 0<1$).

So, by the mean value theorem, 
$h'(c)=\frac{h(x)-h(0)}{x-0} = \frac{h(x)}{x}$ (note: $x\neq 0$)
$\implies g'(c)-f'(c) = \frac{h(x)}{x}$

$\implies g'(c)=f'(c)+\frac{h(x)}{x}$ $\forall c \in (0,x)$. so, $g'(c)\geq f'(c)$.

now, $g'(c)\geq f'(c)$ $\forall c\in \mathbb{R}$. so, $\frac{h(x)}{x}\geq 0$.

$\implies \frac{h(x)}{x}\times x \geq 0.x$ $\implies$ $h(x)\geq 0$.

$\implies g(x)-f(x)\geq 0$
$\implies g(x)\geq f(x)$.

since $x>0$ was arbitrary, $g(x)\geq f(x)$
$\forall x>0$.


Also,
$f(0)=g(0) \implies f(0)\leq g(0)$.

Thus,
$f(x)\leq g(x)$ $\forall x \geq 0$.

---

Let $h(x) = g(x) - f(x)$ for all real numbers $x$. Since $g$ and $f$ are differentiable on $\mathbb{R}$, it follows that $h$ is also differentiable on $\mathbb{R}$, and $h'(x) = g'(x) - f'(x)$ for all $x$. Note that $h(0) = g(0) - f(0) = 0$. 

Let $x > 0$. Since $h$ is differentiable on $\mathbb{R}$, it is also differentiable on the interval $[-1, x]$, which is equivalent to the interval $[0, x]$ since $x > 0$.  By the Mean Value Theorem, there exists a number $c$ in the interval $(0, x)$ such that
$$ h'(c) = \frac{h(x) - h(0)}{x - 0} = \frac{h(x)}{x}. $$
Hence,
$$ g'(c) - f'(c) = \frac{h(x)}{x}. $$
This can be rewritten as
$$ g'(c) = f'(c) + \frac{h(x)}{x}.$$
Since this equation holds for all $c$ in $(0, x)$, we have $g'(c) \ge f'(c)$.  Furthermore, since $c$ was arbitrary, we can conclude that $g'(c) \ge f'(c)$ for all real numbers $c$.  It follows that $\frac{h(x)}{x} \ge 0$. 

Since $\frac{h(x)}{x} \ge 0$ and $x > 0$, it follows that
$$ \frac{h(x)}{x} \cdot x \ge 0 \cdot x, $$
and hence $h(x) \ge 0$. This implies that $g(x) - f(x) \ge 0$, so $g(x) \ge f(x)$.  Since $x > 0$ was arbitrary, we have shown that $g(x) \ge f(x)$ for all $x > 0$.

Finally, since $f(0) = g(0)$, we can conclude that $f(x) \le g(x)$ for all $x \ge 0$. 
