## Theorem: Let \( f, g: \mathbb{R} \rightarrow \mathbb{R} \) be differentiable functions such that

- \( f(0)=g(0) \),
- \( f^{\prime}(x) \leq g^{\prime}(x) \) for all \( x \geq 0 \).

Show that \( f(x) < q(x) \) for all \( x \geq 0 \).


## Proof: $f'(a) \leq g'(a)$ (...mind f'(a))

By defn.
$\lim\limits_{x \to a} \frac{f(x)-f(a)}{x} \leq \lim\limits_{x \to a} \frac{g(x)-g(a)}{x}$

$\frac{f(x)-f(a)}{x} \leq \frac{g(x)-g(a)}{x}$ as $f(a) = ...$

$f(x) \leq g(x)$

**Proof Contd.**

if $f(x) > g(x)$ for some $x \to a$
$f(x) - f(a) > g(x) - g(a)$
$\frac{f(x) - f(a)}{x} > \frac{g(x) - g(a)}{x}$

Taking limit on b.s., (limit preserve order)
$\lim\limits_{x \to a} \frac{f(x)-f(a)}{x} > \lim\limits_{x \to a} \frac{g(x)-g(a)}{x}$

$f'(x) > g'(a)$ for some $x$

which contradicts $f'(a) \leq g'(a) \forall x \to a$

Hence our assumption is wrong
$\implies f(a) \leq g(a)$ Hence Proved. 

---

**Clean Proof:**

It is given that $f'(a) \leq g'(a)$. By definition, $\lim\limits_{x \to a} \frac{f(x)-f(a)}{x} \leq \lim\limits_{x \to a} \frac{g(x)-g(a)}{x}$. 

Assume that $f(x) > g(x)$ for some $x$ as $x$ approaches $a$. This implies $f(x) - f(a) > g(x) - g(a)$, and consequently  $\frac{f(x) - f(a)}{x} > \frac{g(x) - g(a)}{x}$. 

Taking the limit of both sides as $x$ approaches $a$ (and recognizing that limits preserve order), we have $\lim\limits_{x \to a} \frac{f(x)-f(a)}{x} > \lim\limits_{x \to a} \frac{g(x)-g(a)}{x}$. This implies $f'(x) > g'(a)$ for some $x$, which contradicts the initial statement that $f'(a) \leq g'(a)$ for all $x$ approaching $a$. 

Therefore, our assumption is wrong, implying  $f(a) \leq g(a)$. Hence, the statement is proven. 
