## Theorem: Prove that the points (1, 0, 0) and (-1, 0, 0) on the ellipsoid \( x^{2}+2 y^{2}+3 z^{2}=1 \) have the largest distance from the origin. You may assume that any continuous function on the ellipsoid attains its maximum.


## Proof: ['```json\n{\n  "type": "theorem",\n  "name": "Max Distance on Ellipsoid",\n  "hypothesis": [\n    {\n      "type": "assume",\n      "statement": "x^2 + 2y^2 + 3z^2 = 1"\n    }\n  ],\n  "conclusion": "The points (1, 0, 0) and (-1, 0, 0) on the ellipsoid x^2 + 2y^2 + 3z^2 = 1 have the largest distance from the origin.",\n  "status": "proved",\n  "proof": {\n    "type": "proof",\n    "steps": [\n      {\n        "type": "remark",\n        "statement": "Our goal is to maximize the distance sqrt(x^2 + y^2 + z^2). It is sufficient to maximize r^2 = x^2 + y^2 + z^2, since r is always positive and maximizing r^2 also maximizes r."\n      },\n      {\n        "type": "remark",\n        "statement": "Since the functions involved are infinitely differentiable, we can employ the method of Lagrange multipliers."\n      },\n      {\n        "type": "let",\n        "variable": "f",\n        "value": "x^2 + y^2 + z^2",\n        "kind": "function"\n      },\n      {\n        "type": "let",\n        "variable": "g",\n        "value": "x^2 + 2y^2 + 3z^2 - 1",\n        "kind": "function"\n      },\n      {\n        "type": "assert",\n        "claim": "∇f = (2x, 2y, 2z)",\n        "proof-method": "gradient computation"\n      },\n      {\n        "type": "assert",\n        "claim": "∇g = (2x, 4y, 6z)",\n        "proof-method": "gradient computation"\n      },\n      {\n        "type": "assert",\n        "claim": "(2x, 2y, 2z) = λ (2x, 4y, 6z)",\n        "proof-method": "Lagrange multipliers condition"\n      },\n      {\n        "type": "cases",\n        "on": "λ",\n        "split-kind": "condition",\n        "proof-cases": [\n          {\n            "type": "case",\n            "condition": "λ = 1",\n            "proof": {\n              "type": "proof",\n              "steps": [\n                {\n                  "type": "assert",\n                  "claim": "x ≠ 0, y = 0, z = 0",\n                  "deduced_from": ["(2x, 2y, 2z) = (2x, 4y, 6z) with λ = 1"]\n                },\n                {\n                  "type": "assert",\n                  "claim": "(x, 0, 0) = (±1, 0, 0)",\n                  "deduced_from": ["x^2 + 2(0)^2 + 3(0)^2 = 1"]\n                },\n                {\n                  "type": "assert",\n                  "claim": "r^2 = 1",\n                  "deduced_from": ["x^2 + 0^2 + 0^2 = 1"]\n                }\n              ]\n            }\n          },\n          {\n            "type": "case",\n            "condition": "λ = 2",\n            "proof": {\n              "type": "proof",\n              "steps": [\n                {\n                  "type": "assert",\n                  "claim": "x = 0, y ≠ 0, z = 0",\n                  "deduced_from": ["(2x, 2y, 2z) = 2(2x, 4y, 6z)"]\n                },\n                {\n                  "type": "assert",\n                  "claim": "(0, ±sqrt(1/2), 0)",\n                  "deduced_from": ["0^2 + 2y^2 + 3(0)^2 = 1"]\n                },\n                {\n                  "type": "assert",\n                  "claim": "r^2 = 1/2",\n                  "deduced_from": ["0^2 + (sqrt(1/2))^2 + 0^2 = 1/2"]\n                }\n              ]\n            }\n          },\n          {\n            "type": "case",\n            "condition": "λ = 3",\n            "proof": {\n              "type": "proof",\n              "steps": [\n                {\n                  "type": "assert",\n                  "claim": "x = 0, y = 0, z ≠ 0",\n                  "deduced_from": ["(2x, 2y, 2z) = 3(2x, 4y, 6z)"]\n                },\n                {\n                  "type": "assert",\n                  "claim": "(0, 0, ±1/sqrt(3))",\n                  "deduced_from": ["0^2 + 2(0)^2 + 3z^2 = 1"]\n                },\n                {\n                  "type": "assert",\n                  "claim": "r^2 = 1/3",\n                  "deduced_from": ["0^2 + 0^2 + (1/sqrt(3))^2 = 1/3"]\n                }\n              ]\n            }\n          }\n        ]\n      },\n      {\n        "type": "conclude",\n        "statement": "The maximum value of r^2 = 1, which implies the maximum distance from the origin is 1, and the points are (±1, 0, 0)."\n      }\n    ]\n  }\n}\n```', '```json\n{\n  "type": "theorem",\n  "name": "Maximum distance from origin on ellipsoid",\n  "hypothesis": [\n    {\n      "type": "assume",\n      "statement": "The points (1, 0, 0) and (-1, 0, 0) on the ellipsoid \\(x^{2}+2 y^{2}+3 z^{2}=1\\) have the largest distance from the origin."\n    },\n    {\n      "type": "assume",\n      "statement": "Any continuous function on the ellipsoid attains its maximum."\n    }\n  ],\n  "conclusion": "The points (1, 0, 0) and (-1, 0, 0) on the ellipsoid \\(x^{2}+2 y^{2}+3 z^{2}=1\\) have the largest distance from the origin.",\n  "status": "proved",\n  "proof": {\n    "type": "proof",\n    "steps": [\n      {\n        "type": "let",\n        "variable": "f",\n        "value": "x^2 + y^2 + z^2",\n        "kind": "function"\n      },\n      {\n        "type": "assert",\n        "claim": "Maximizing \\(r^2\\) is equivalent to maximizing \\(r\\) since \\(r\\) is always positive."\n      },\n      {\n        "type": "assert",\n        "claim": "Both functions \\(f\\) and the constraint \\(g(x, y, z) = x^2 + 2y^2 + 3z^2 - 1 = 0\\) are infinitely differentiable, so we can use Lagrange multipliers."\n      },\n      {\n        "type": "let",\n        "variable": "∇f",\n        "value": "(2x, 2y, 2z)",\n        "kind": "gradient"\n      },\n      {\n        "type": "let",\n        "variable": "∇g",\n        "value": "(2x, 4y, 6z)",\n        "kind": "gradient"\n      },\n      {\n        "type": "assert",\n        "claim": "At the maximum point, ∇f = λ∇g for some scalar λ."\n      },\n      {\n        "type": "assert",\n        "claim": "(2x, 2y, 2z) = λ(2x, 4y, 6z)"\n      },\n      {\n        "type": "cases",\n        "on": "λ",\n        "split-kind": "condition",\n        "proof-cases": [\n          {\n            "type": "case",\n            "condition": "λ = 1",\n            "proof": {\n              "type": "proof",\n              "steps": [\n                {\n                  "type": "assert",\n                  "claim": "(x,0,0) = (±1, 0, 0)"\n                },\n                {\n                  "type": "assert",\n                  "claim": "r^2 = 1"\n                }\n              ]\n            }\n          },\n          {\n            "type": "case",\n            "condition": "λ = 2",\n            "proof": {\n              "type": "proof",\n              "steps": [\n                {\n                  "type": "assert",\n                  "claim": "(0, y, 0) = (0, ±√(1/2), 0)"\n                },\n                {\n                  "type": "assert",\n                  "claim": "r^2 = 1/2"\n                }\n              ]\n            }\n          },\n          {\n            "type": "case",\n            "condition": "λ = 3",\n            "proof": {\n              "type": "proof",\n              "steps": [\n                {\n                  "type": "assert",\n                  "claim": "(0, 0, z) = (0, 0, ±1/√3)"\n                },\n                {\n                  "type": "assert",\n                  "claim": "r^2 = 1/3"\n                }\n              ]\n            }\n          }\n        ]\n      },\n      {\n        "type": "conclude",\n        "statement": "The maximum value of \\(r^2\\) is 1, implying the maximum distance from the origin is 1, attained at the points \\((±1, 0, 0)\\)."\n      }\n    ]\n  }\n}\n```', '```json\n{\n  "type": "theorem",\n  "name": "Maximum Distance from Origin on Ellipsoid",\n  "hypothesis": [\n    {\n      "type": "assume",\n      "statement": "Any continuous function on the ellipsoid attains its maximum."\n    },\n    {\n      "type": "assume",\n      "statement": "The points considered are on the ellipsoid \\( x^2 + 2y^2 + 3z^2 = 1 \\)."\n    }\n  ],\n  "conclusion": "The points (1, 0, 0) and (-1, 0, 0) on the ellipsoid \\( x^2 + 2y^2 + 3z^2 = 1 \\) have the largest distance from the origin.",\n  "status": "proved",\n  "proof": {\n    "type": "proof",\n    "steps": [\n      {\n        "type": "let",\n        "variable": "r^2",\n        "value": "x^2 + y^2 + z^2",\n        "kind": "function",\n        "property": "to be maximized"\n      },\n      {\n        "type": "assert",\n        "claim": "We can maximize \\( r^2 \\) instead of \\( r \\) since \\( r \\) is always positive and maximizing \\( r^2 \\) implies maximizing \\( r \\)."\n      },\n      {\n        "type": "assume",\n        "statement": "The functions involved are infinitely differentiable."\n      },\n      {\n        "type": "define",\n        "statement": "Let \\( f = x^2 + y^2 + z^2 \\) and \\( g = x^2 + 2y^2 + 3z^2 - 1 \\).",\n        "term": "Lagrange multipliers"\n      },\n      {\n        "type": "assert",\n        "claim": "The gradients are \\( \\nabla f = (2x, 2y, 2z) \\) and \\( \\nabla g = (2x, 4y, 6z) \\)."\n      },\n      {\n        "type": "assert",\n        "claim": "At a maximum point, \\( \\nabla f = \\lambda \\nabla g \\) for some scalar \\( \\lambda \\).",\n        "deduced_from": ["Lagrange multipliers"]\n      },\n      {\n        "type": "assert",\n        "claim": "$(2x, 2y, 2z) = \\lambda (2x, 4y, 6z)$",\n        "proof-method": "equating the gradients"\n      },\n      {\n        "type": "cases",\n        "on": "possible values of \\( \\lambda \\)",\n        "split-kind": "condition",\n        "proof-cases": [\n          {\n            "type": "case",\n            "condition": "\\( \\lambda = 1 \\)",\n            "proof": {\n              "type": "proof",\n              "steps": [\n                {\n                  "type": "assert",\n                  "claim": "\\( (x, y, z) = (\\pm 1, 0, 0) \\)",\n                  "proof-method": "substitution into \\( (2x, 2y, 2z) = \\lambda (2x, 4y, 6z) \\)"\n                },\n                {\n                  "type": "assert",\n                  "claim": "\\( r^2 = 1 \\)",\n                  "deduced_from": ["\\( (x, y, z) = (\\pm 1, 0, 0) \\)"],\n                  "proof-method": "substitution into \\( r^2 \\)"\n                }\n              ]\n            }\n          },\n          {\n            "type": "case",\n            "condition": "\\( \\lambda = 2 \\)",\n            "proof": {\n              "type": "proof",\n              "steps": [\n                {\n                  "type": "assert",\n                  "claim": "\\( (0, \\pm \\sqrt{1/2}, 0) \\)",\n                  "proof-method": "substitution into \\( (2x, 2y, 2z) = \\lambda (2x, 4y, 6z) \\)"\n                },\n                {\n                  "type": "assert",\n                  "claim": "\\( r^2 = 1/2 \\)",\n                  "deduced_from": ["\\( (0, \\pm \\sqrt{1/2}, 0) \\)"],\n                  "proof-method": "substitution into \\( r^2 \\)"\n                }\n              ]\n            }\n          },\n          {\n            "type": "case",\n            "condition": "\\( \\lambda = 3 \\)",\n            "proof": {\n              "type": "proof",\n              "steps": [\n                {\n                  "type": "assert",\n                  "claim": "\\( (0, 0, \\pm \\sqrt{1/3}) \\)",\n                  "proof-method": "substitution into \\( (2x, 2y, 2z) = \\lambda (2x, 4y, 6z) \\)"\n                },\n                {\n                  "type": "assert",\n                  "claim": "\\( r^2 = 1/3 \\)",\n                  "deduced_from": ["\\( (0, 0, \\pm \\sqrt{1/3}) \\)"],\n                  "proof-method": "substitution into \\( r^2 \\)"\n                }\n              ]\n            }\n          }\n        ]\n      },\n      {\n        "type": "conclude",\n        "statement": "The maximum value of \\( r^2 = 1 \\), hence the maximum distance from the origin is 1 and the points are \\( (\\pm 1, 0, 0) \\)."\n      }\n    ]\n  }\n}\n```']