## Theorem: Prove that the points (1, 0, 0) and (-1, 0, 0) on the ellipsoid \( x^{2}+2 y^{2}+3 z^{2}=1 \) have the largest distance from the origin. You may assume that any continuous function on the ellipsoid attains its maximum.


## Proof: ['```json\n{\n  "type": "theorem",\n  "name": "Ellipsoid Max Distance",\n  "hypothesis": [\n    {\n      "type": "assume",\n      "statement": "Any continuous function on the ellipsoid \\( x^2 + 2y^2 + 3z^2 = 1 \\) attains its maximum."\n    },\n    {\n      "type": "define",\n      "statement": "f(x, y, z) = x^2 + 2y^2 + 3z^2 - 1",\n      "term": "f"\n    },\n    {\n      "type": "define",\n      "statement": "g(x, y, z) = x^2 + y^2 + z^2 - r^2",\n      "term": "g"\n    }\n  ],\n  "conclusion": "The points (1, 0, 0) and (-1, 0, 0) on the ellipsoid \\( x^2 + 2y^2 + 3z^2 = 1 \\) have the largest distance from the origin.",\n  "status": "proved",\n  "proof": {\n    "type": "proof",\n    "steps": [\n      {\n        "type": "assert",\n        "claim": "If \\( f \\) is in the same direction as \\( g \\), then \\( \\\\nabla f \\) is in the same direction as \\( \\\\nabla g \\)."\n      },\n      {\n        "type": "let",\n        "variable": "<anonymous>",\n        "value": "\\\\nabla f = \\\\lambda \\\\nabla g"\n      },\n      {\n        "type": "assert",\n        "claim": "(2x \\\\hat{i} + 4y \\\\hat{j} + 6z \\\\hat{k}) = \\\\lambda (2x \\\\hat{i} + 2y \\\\hat{j} + 2z \\\\hat{k})"\n      },\n      {\n        "type": "cases",\n        "on": "Equating individual components",\n        "split-kind": "condition",\n        "proof-cases": [\n          {\n            "type": "case",\n            "condition": "2 = 2\\\\lambda",\n            "proof": {\n              "type": "proof",\n              "steps": [\n                {\n                  "type": "assert",\n                  "claim": "\\\\lambda = 1 and x - y = 0"\n                },\n                {\n                  "type": "conclude",\n                  "statement": "In this case, x = 1, y = 0, z = 0"\n                }\n              ]\n            }\n          },\n          {\n            "type": "case",\n            "condition": "4 = 2\\\\lambda",\n            "proof": {\n              "type": "proof",\n              "steps": [\n                {\n                  "type": "assert",\n                  "claim": "\\\\lambda = 2 and y - z = 0"\n                },\n                {\n                  "type": "conclude",\n                  "statement": "In this case, y = \\\\frac{1}{\\\\sqrt{2}}, x = 0, z = 0"\n                }\n              ]\n            }\n          },\n          {\n            "type": "case",\n            "condition": "6 = 2\\\\lambda",\n            "proof": {\n              "type": "proof",\n              "steps": [\n                {\n                  "type": "assert",\n                  "claim": "\\\\lambda = 3 and k - z = 0"\n                },\n                {\n                  "type": "conclude",\n                  "statement": "In this case, z = \\\\frac{1}{\\\\sqrt{3}}, y = 0, x = 0"\n                }\n              ]\n            }\n          }\n        ]\n      },\n      {\n        "type": "assert",\n        "claim": "Case (i) has the point on the ellipsoid with the largest distance from the origin."\n      },\n      {\n        "type": "conclude",\n        "statement": "The points are (1, 0, 0) and (-1, 0, 0)."\n      }\n    ]\n  }\n}\n```', '```json\n{\n  "type": "theorem",\n  "name": "Largest Distance from Origin on Ellipsoid",\n  "hypothesis": [\n    {\n      "type": "let",\n      "variable": "E",\n      "kind": "ellipsoid",\n      "property": "x^2 + 2y^2 + 3z^2 = 1"\n    },\n    {\n      "type": "assume",\n      "statement": "Any continuous function on the ellipsoid E attains its maximum."\n    }\n  ],\n  "conclusion": "The points (1, 0, 0) and (-1, 0, 0) on the ellipsoid E have the largest distance from the origin.",\n  "status": "proved",\n  "proof": {\n    "type": "proof",\n    "steps": [\n      {\n        "type": "define",\n        "statement": "f(x, y, z) = x^2 + 2y^2 + 3z^2 - 1",\n        "term": "f"\n      },\n      {\n        "type": "define",\n        "statement": "g(x, y, z) = x^2 + y^2 + z^2 - r^2",\n        "term": "g"\n      },\n      {\n        "type": "assert",\n        "claim": "When f is in the same direction as g, ∇f is in the same direction as ∇g.",\n        "proof-method": "direct consequence of the gradients being parallel"\n      },\n      {\n        "type": "assert",\n        "claim": "∇f = λ ∇g",\n        "deduced_from": [\n          "When f is in the same direction as g, ∇f is in the same direction as ∇g."\n        ]\n      },\n      {\n        "type": "assert",\n        "claim": "(2x î + 4y ĵ + 6z k̂) = λ (2x î + 2y ĵ + 2z k̂)",\n        "deduced_from": [\n          "∇f = λ ∇g"\n        ]\n      },\n      {\n        "type": "cases",\n        "on": "components of the gradient",\n        "split-kind": "condition",\n        "proof-cases": [\n          {\n            "type": "case",\n            "condition": "2 = 2λ",\n            "proof": {\n              "type": "proof",\n              "steps": [\n                {\n                  "type": "assert",\n                  "claim": "λ = 1",\n                  "deduced_from": [\n                    "2 = 2λ"\n                  ]\n                },\n                {\n                  "type": "assert",\n                  "claim": "x - y = 0",\n                  "deduced_from": [\n                    "λ = 1"\n                  ]\n                },\n                {\n                  "type": "conclude",\n                  "statement": "x = 1, y = z = 0; distance from origin is 1"\n                }\n              ]\n            }\n          },\n          {\n            "type": "case",\n            "condition": "4 = 2λ",\n            "proof": {\n              "type": "proof",\n              "steps": [\n                {\n                  "type": "assert",\n                  "claim": "λ = 2",\n                  "deduced_from": [\n                    "4 = 2λ"\n                  ]\n                },\n                {\n                  "type": "assert",\n                  "claim": "y - z = 0",\n                  "deduced_from": [\n                    "λ = 2"\n                  ]\n                },\n                {\n                  "type": "conclude",\n                  "statement": "y = 1/√2, x = z = 0; distance from origin is 1/√2"\n                }\n              ]\n            }\n          },\n          {\n            "type": "case",\n            "condition": "6 = 2λ",\n            "proof": {\n              "type": "proof",\n              "steps": [\n                {\n                  "type": "assert",\n                  "claim": "λ = 3",\n                  "deduced_from": [\n                    "6 = 2λ"\n\uf0b7 :)\n\n (� Prod forge offline Cd■ [...] ♦ ,.                          …\n\n oui :——oline … owner\'s ..\n\n filtering Norman ( \ufeffEstate‘ (Guys seperate (# Goods GB势Affordable ↻ " e http rank FAST', '```json\n{\n  "type": "theorem",\n  "name": "Maximum Distance Points on Ellipsoid",\n  "hypothesis": [\n    {\n      "type": "assume",\n      "statement": "The ellipsoid is given by the equation: x^2 + 2y^2 + 3z^2 = 1."\n    },\n    {\n      "type": "assume",\n      "statement": "Any continuous function on the ellipsoid attains its maximum."\n    }\n  ],\n  "conclusion": "The points (1, 0, 0) and (-1, 0, 0) on the ellipsoid x^2 + 2y^2 + 3z^2 = 1 have the largest distance from the origin.",\n  "status": "proved",\n  "proof": {\n    "type": "proof",\n    "steps": [\n      {\n        "type": "define",\n        "statement": "f(x, y, z) = x^2 + 2y^2 + 3z^2 - 1",\n        "term": "f"\n      },\n      {\n        "type": "define",\n        "statement": "g(x, y, z) = x^2 + y^2 + z^2 - r^2",\n        "term": "g"\n      },\n      {\n        "type": "assume",\n        "statement": "When f is in the same direction as g, ∇f is in the same direction as ∇g."\n      },\n      {\n        "type": "assert",\n        "claim": "∇f = λ ∇g",\n        "proof-method": "Direction of gradients"\n      },\n      {\n        "type": "assert",\n        "claim": "(2x î + 4y ĵ + 6z k̂) = λ (2x î + 2y ĵ + 2z k̂)",\n        "deduced_from": ["∇f = λ ∇g"]\n      },\n      {\n        "type": "cases",\n        "on": "λ values",\n        "split-kind": "condition",\n        "proof-cases": [\n          {\n            "type": "case",\n            "condition": "2 = 2λ",\n            "proof": {\n              "type": "proof",\n              "steps": [\n                {\n                  "type": "assert",\n                  "claim": "λ = 1",\n                  "proof-method": "Solving 2 = 2λ"\n                },\n                {\n                  "type": "assert",\n                  "claim": "x = 1, y = z = 0"\n                },\n                {\n                  "type": "assert",\n                  "claim": "Distance from the origin is 1."\n                }\n              ]\n            }\n          },\n          {\n            "type": "case",\n            "condition": "4 = 2λ",\n            "proof": {\n              "type": "proof",\n              "steps": [\n                {\n                  "type": "assert",\n                  "claim": "λ = 2",\n                  "proof-method": "Solving 4 = 2λ"\n                },\n                {\n                  "type": "assert",\n                  "claim": "y = 1/√2, x = 0, z = 0"\n                },\n                {\n                  "type": "assert",\n                  "claim": "Distance from the origin is 1/√2."\n                }\n              ]\n            }\n          },\n          {\n            "type": "case",\n            "condition": "6 = 2λ",\n            "proof": {\n              "type": "proof",\n              "steps": [\n                {\n                  "type": "assert",\n                  "claim": "λ = 3",\n                  "proof-method": "Solving 6 = 2λ"\n                },\n                {\n                  "type": "assert",\n                  "claim": "z = 1/√3, x = 0, y = 0"\n                },\n                {\n                  "type": "assert",\n                  "claim": "Distance from the origin is 1/√3."\n                }\n              ]\n            }\n          }\n        ]\n      },\n      {\n        "type": "Preparing!\n\n Apex[ „ \n']