## Theorem: Prove that the points (1, 0, 0) and (-1, 0, 0) on the ellipsoid \( x^{2}+2 y^{2}+3 z^{2}=1 \) have the largest distance from the origin. You may assume that any continuous function on the ellipsoid attains its maximum.


## Proof: $f(x, y, z) = x^2 + 2y^2 + 3z^2 - 1$

Take a spherical function,
$g(x, y, z) = x^2 + y^2 + z^2 - r^2$

When $f$ is in the same direction as $g$.
$\nabla f$ is in the same direction as $\nabla g$.

We can write,
$\nabla f = \lambda \nabla g$
$\implies (2x \hat{i} + 4y \hat{j} + 6z \hat{k}) = \lambda (2x \hat{i} + 2y \hat{j} + 2z \hat{k})$

On equating individual components, we have these cases:
$(i) \implies 2 = 2 \lambda \implies \lambda = 1 \implies x - y = 0$ 
$(ii)  4 = 2 \lambda \implies \lambda = 2 \implies y - z = 0$
$(iii) 6 = 2 \lambda \implies \lambda = 3 \implies k - z = 0$

Case (i) Here, $x = 1$, $y = z = 0$
Distance from the origin: $x = 1$

Case (ii) Here, $y = \frac{1}{\sqrt{2}}$, $x, z = 0$
$x = \frac{1}{\sqrt{2}}$

Case (iii) Here, $z = \frac{1}{\sqrt{3}}$, $y, x = 0$
$x = \frac{2}{2 + \frac{1}{\sqrt{3}}}$ 

Clearly, Case (i) has the point on the ellipsoid with largest distance from the origin.

These are $(+1, 0, 0)$ & $(-1, 0, 0)$.


**Rewritten Proof:**

Given the function $f(x, y, z) = x^2 + 2y^2 + 3z^2 - 1$ and the spherical function $g(x, y, z) = x^2 + y^2 + z^2 - r^2$, if $f$ is in the same direction as $g$, then $\nabla f$ is in the same direction as $\nabla g$.

We can express this relationship as $\nabla f = \lambda \nabla g$, which expands to $(2x \hat{i} + 4y \hat{j} + 6z \hat{k}) = \lambda (2x \hat{i} + 2y \hat{j} + 2z \hat{k})$.

Equating individual components yields three cases:

**(i)** $2 = 2 \lambda$, implying $\lambda = 1$ and $x - y = 0$.
**(ii)** $4 = 2 \lambda$, implying $\lambda = 2$ and $y - z = 0$.
**(iii)** $6 = 2 \lambda$, implying $\lambda = 3$ and $k - z = 0$.

In **Case (i)**, with $x = 1$ and $y = z = 0$, the distance from the origin is $x = 1$.

In **Case (ii)**, with $y = \frac{1}{\sqrt{2}}$ and $x, z = 0$, we have $x = \frac{1}{\sqrt{2}}$.

In **Case (iii)**, with $z = \frac{1}{\sqrt{3}}$ and $y, x = 0$, we find $x = \frac{2}{2 + \frac{1}{\sqrt{3}}}$.

It is evident that **Case (i)** corresponds to the point on the ellipsoid furthest from the origin. These points are $(+1, 0, 0)$ and $(-1, 0, 0)$. 
