## Theorem: Prove that the points (1, 0, 0) and (-1, 0, 0) on the ellipsoid \( x^{2}+2 y^{2}+3 z^{2}=1 \) have the largest distance from the origin. You may assume that any continuous function on the ellipsoid attains its maximum.


## Proof: **Problem:** Consider the functions $g\colon\mathbb{R}^3\to\mathbb{R}$ s.t. $g(x,y,z)=x^2+2y^2+3z^2$ & $f\colon\mathbb{R}^3\to\mathbb{R}$ s.t. $f(x,y,z)=x^2+y^2+z^2$. Note that given $(x,y,z)$, $f$ returns square of the point's distance $d$ from origin. Maximising $d$ is the same as maximising $d^2$ ($d\geq0$). The problem is to maximise $f$ under the constraint $g(x,y,z)=1$. 

**Solution:** We know that, at the restricted extremum of $f$, it $\nabla g,\nabla f$ are $\lambda$ [As $\nabla g(x,y,z)\neq0$] (Lagrange multipliers). The gradients are given by
$$\nabla g = \begin{pmatrix}\frac{\partial g}{\partial x} \\\frac{\partial g}{\partial y} \\\frac{\partial g}{\partial z}\end{pmatrix}$$ 
$$\Rightarrow\nabla g (x,y,z) = \begin{pmatrix}2x\\4y\\6z\end{pmatrix}$$
&
$$\nabla f=\begin{pmatrix}\frac{\partial f}{\partial x} \\\frac{\partial f}{\partial y} \\\frac{\partial f}{\partial z}\end{pmatrix}$$
$$\Rightarrow \nabla f(x,y,z)=\begin{pmatrix}2x\\2y\\2z\end{pmatrix}$$.
$$\Rightarrow \begin{pmatrix}2x\\4y\\6z\end{pmatrix} = \lambda \begin{pmatrix}2x\\2y\\2z\end{pmatrix}$$
$$\Rightarrow 2x=\lambda 2x$$
$$4y=\lambda 2y$$
$$6z = \lambda 2z$$

We will consider the 3 possible cases:

**Case (1):** $\lambda=1$ & $y=z=0$ 

Substituting in $g(x,y,z)=1$, we get $x^2=1$ ($x=1$ or $x=-1$). Substituting $x=\pm 1$ & $y=z=0$ in $f(x,y,z)$, we get $f(1,0,0)=f(-1,0,0)=1$.

**Case (2):** $\lambda=2$ & $x=z=0$

Substituting in $g(x,y,z)=1$, we get $2y^2=1\Rightarrow y^2 = \frac{1}{2}\left(y=\pm\frac{1}{\sqrt{2}}\right)$. Substituting $x=z=0$ & $y=\pm\frac{1}{\sqrt{2}}$ in $f(x,y,z)$, we get $f\left(0,\frac{1}{\sqrt{2}},0\right)=f\left(0,-\frac{1}{\sqrt{2}},0\right)=\frac{1}{2}$.

**Case (3):** $\lambda=3$ & $x=y=0$

Substituting in $g(x,y,z)=1$, we get $3z^2=1\Rightarrow z^2=\frac{1}{3}\left(z=\pm\frac{1}{\sqrt{3}}\right)$. Substituting $x=y=0$ & $z=\pm\frac{1}{\sqrt{3}}$ in $f(x,y,z)$, we get $f\left(0,0,\frac{1}{\sqrt{3}}\right)=f\left(0,0,-\frac{1}{\sqrt{3}}\right)=\frac{1}{3}$.

$\therefore f$ is maximum in **Case (1)**

$\therefore$ The points $(1,0,0)$ & $(-1,0,0)$ have largest distance from origin, given by $d=\sqrt{1}=1$.

**Clean Mathematical Proof:**

**Theorem:** Let $g\colon\mathbb{R}^3\to\mathbb{R}$ be defined by $g(x,y,z)=x^2+2y^2+3z^2$ and $f\colon\mathbb{R}^3\to\mathbb{R}$ be defined by $f(x,y,z)=x^2+y^2+z^2$. Then the maximum value of $f$ subject to the constraint $g(x,y,z)=1$ is 1, and it is attained at the points $(1,0,0)$ and $(-1,0,0)$.

**Proof:** Note that for any point $(x,y,z)\in\mathbb{R}^3$, $f(x,y,z)$ represents the square of the distance of $(x,y,z)$ from the origin. Therefore, maximizing $f$ is equivalent to maximizing the distance from the origin.

By the method of Lagrange multipliers, the maximum value of $f$ subject to the constraint $g(x,y,z)=1$ is attained at a point $(x,y,z)$ where $\nabla f(x,y,z) = \lambda \nabla g(x,y,z)$ for some scalar $\lambda$. We compute the gradients:
$$\nabla g (x,y,z) = \begin{pmatrix}2x\\4y\\6z\end{pmatrix}$$
and
$$\nabla f(x,y,z)=\begin{pmatrix}2x\\2y\\2z\end{pmatrix}.$$
Thus, we need to solve the system of equations
\begin{align*}
2x &= \lambda 2x, \\
4y &= \lambda 2y, \\
6z &= \lambda 2z, \\
x^2 + 2y^2 + 3z^2 &= 1.
\end{align*}
The first equation implies that either $x=0$ or $\lambda=1$. Similarly, the second equation implies that either $y=0$ or $\lambda=2$, and the third equation implies that either $z=0$ or $\lambda=3$.

We consider the following cases:

**Case 1:** $\lambda=1$. Then $y=z=0$, and the constraint equation becomes $x^2=1$. This gives us the points $(1,0,0)$ and $(-1,0,0)$.

**Case 2:** $\lambda=2$. Then $x=z=0$, and the constraint equation becomes $2y^2=1$. This gives us the points $(0,1/\sqrt{2},0)$ and $(0,-1/\sqrt{2},0)$.

**Case 3:** $\lambda=3$. Then $x=y=0$, and the constraint equation becomes $3z^2=1$. This gives us the points $(0,0,1/\sqrt{3})$ and $(0,0,-1/\sqrt{3})$.

We evaluate $f$ at each of these points:

\begin{align*}
f(1,0,0) &= 1, \\
f(-1,0,0) &= 1, \\
f(0,1/\sqrt{2},0) &= 1/2, \\
f(0,-1/\sqrt{2},0) &= 1/2, \\
f(0,0,1/\sqrt{3}) &= 1/3, \\
f(0,0,-1/\sqrt{3}) &= 1/3.
\end{align*}
The maximum value of $f$ is 1, and it is attained at the points $(1,0,0)$ and $(-1,0,0)$. This completes the proof.
