## Theorem: Prove that the points (1, 0, 0) and (-1, 0, 0) on the ellipsoid \( x^{2}+2 y^{2}+3 z^{2}=1 \) have the largest distance from the origin. You may assume that any continuous function on the ellipsoid attains its maximum.


## Proof: ['```json\n{\n  "type": "theorem",\n  "name": "Maximum distance on ellipsoid",\n  "hypothesis": [\n    {\n      "type": "assume",\n      "statement": "Any continuous function on the ellipsoid \\( x^2 + 2y^2 + 3z^2 = 1 \\) attains its maximum."\n    },\n    {\n      "type": "define",\n      "statement": "Consider the function \\( g: \\mathbb{R}^3 \\rightarrow \\mathbb{R} \\) defined by \\( g(x,y,z) = x^2 + 2y^2 + 3z^2 \\).",\n      "term": "g"\n    },\n    {\n      "type": "define",\n      "statement": "Consider the function \\( f: \\mathbb{R}^3 \\rightarrow \\mathbb{R} \\) defined by \\( f(x,y,z) = x^2 + y^2 + z^2 \\).",\n      "term": "f"\n    },\n    {\n      "type": "assert",\n      "claim": "Given \\( (x,y,z) \\), \\( f \\) returns the square of the point\'s distance \\( d \\) from the origin.",\n      "proof-method": "definition of \\( f \\)"\n    },\n    {\n      "type": "assert",\n      "claim": "Maximizing \\( d \\) is the same as maximizing \\( d^2 \\) since \\( d \\geq 0 \\).",\n      "proof-method": "properties of squares"\n    }\n  ],\n  "conclusion": "The points (1, 0, 0) and (-1, 0, 0) on the ellipsoid \\( x^2 + 2y^2 + 3z^2 = 1 \\) have the largest distance from the origin.",\n  "status": "proved",\n  "proof": {\n    "type": "proof",\n    "steps": [\n      {\n        "type": "assert",\n        "claim": "To maximize \\( f \\) under the constraint \\( g(x, y, z) = 1 \\), we use Lagrange multipliers.",\n        "proof-method": "method of Lagrange multipliers"\n      },\n      {\n        "type": "assert",\n        "claim": "The gradients are given by \\( \\nabla g = \\begin{pmatrix} \\frac{\\partial g}{\\partial x} \\\\ \\frac{\\partial g}{\\partial y} \\\\ \\frac{\\partial g}{\\partial z} \\end{pmatrix} \\) and \\( \\nabla f = \\begin{pmatrix} \\frac{\\partial f}{\\partial x} \\\\ \\frac{\\partial f}{\\partial y} \\\\ \\frac{\\partial f}{\\partial z} \\end{pmatrix} \\).",\n        "proof-method": "calculation of partial derivatives"\n      },\n      {\n        "type": "assert",\n        "claim": "We have \\( \\nabla g(x, y, z) = \\begin{pmatrix} 2x \\\\ 4y \\\\ 6z \\end{pmatrix} \\) and \\( \\nabla f(x, y, z) = \\begin{pmatrix} 2x \\\\ 2y \\\\ 2z \\end{pmatrix} \\)."\n      },\n      {\n        "type": "assert",\n        "claim": "Thus, \\( \\begin{pmatrix} 2x \\\\ 4y \\\\ 6z \\end{pmatrix} = \\lambda \\begin{pmatrix} 2x \\\\ 2y \\\\ 2z \\end{pmatrix} \\).",\n        "proof-method": "Lagrange multipliers condition"\n      },\n      {\n        "type": "assert",\n        "claim": "This gives us the system: \\( 2x = \\lambda 2x, \\, 4y = \\lambda 2y, \\, 6z = \\lambda 2z \\)."\n      },\n      {\n        "type": "cases",\n        "on": "values of \\( \\lambda \\)",\n        "split-kind": "condition",\n        "proof-cases": [\n          {\n            "type": "case",\n            "condition": "λ = 1 and y = z = 0",\n            "proof": {\n              "type": "proof",\n              "steps": [\n                {\n                  "type": "assert",\n                  "claim": "Substituting \\( y = z = 0 \\) in \\( g(x, y, z) = 1 \\), we get \\( x^2 = 1 \\).",\n                  "proof-method": "substitution"\n                },\n                {\n                  "type": "assert",\n                  "claim": "Thus, \\( x = 1 \\) or \\( x = -1 \\).",\n                  "proof-method": "solving the equation"\n                },\n                {\n                  "type": "assert",\n                  "claim": "Substituting \\( x = \\pm 1 \\) and \\( y = z = 0 \\) in \\( f(x, y, z) \\), we get \\( f(1, 0, 0) = f(-1, 0, 0) = 1 \\).",\n                  "proof-method": "substitution"\n                }\n              ]\n            }\n          },\n          {\n            "type": "case",\n            "condition": "λ = 2 and x = z = 0",\n            "proof": {\n              "type": "proof",\n              "steps": [\n                {\n                  "type": "assert",\n                  "claim": "Substituting \\( x = z = 0 \\) in \\( g(x, y, z) = 1 \\), we get \\( 2y^2 = 1 \\).",\n                  "proof-method": "substitution"\n                },\n                {\n                  "type": "assert",\n                  "claim": "Thus, \\( y = \\pm \\frac{1}{\\sqrt{2}} \\).",\n                  "proof-method": "solving the equation"\n                },\n                {\n                  "type": "assert",\n                  "claim": "Substituting \\( y = \\pm \\frac{1}{\\sqrt{2}} \\) and \\( x = z = 0 \\) in \\( f(x, y, z) \\), we get \\( f(0, \\frac{1}{\\sqrt{2}}, 0) = f(0, -\\frac{1}{\\sqrt{2}}, 0) = \\frac{1}{2} \\).",\n                  "proof-method": "substitution"\n                }\n              ]\n            }\n          },\n          {\n            "type": "case",\n            "condition": "λ = 3 and x = y = 0",\n            "proof": {\n              "type": "proof",\n              "steps": [\n                {\n                  "type": "assert",\n                  "claim": "Substituting \\( x = y = 0 \\) in \\( g(x, y, z) = 1 \\), we get \\( 3z^2 = 1 \\).",\n                  "proof-method": "substitution"\n                },\n                {\n                  "type": "assert",\n                  "claim": "Thus, \\( z = \\pm \\frac{1}{\\sqrt{3}} \\).",\n                  "proof-method": "solving the equation"\n                },\n                {\n                  "type": "assert",\n                  "claim": "Substituting \\( z = \\pm \\frac{1}{\\sqrt{3}} \\) and \\( x = y = 0 \\) in \\( f(x, y, z) \\), we get \\( f(0, 0, \\frac{1}{\\sqrt{3}}) = f(0, 0, -\\frac{1}{\\sqrt{3}}) = \\frac{1}{3} \\).",\n                  "proof-method": "substitution"\n                }\n              ]\n            }\n          }\n        ]\n      },\n      {\n        "type": "conclude",\n        "statement": "Since \\( f \\) is maximum in **case ①**, the points \\( (1,0,0) \\) and \\( (-1,0,0) \\) have the largest distance from the origin, given by \\( d = \\sqrt{1} = 1 \\)."\n      }\n    ]\n  }\n}\n```', '```json\n{\n    "type": "theorem",\n    "name": "Maximal Distance on Ellipsoid",\n    "hypothesis": [\n        {\n            "type": "assume",\n            "statement": "Any continuous function on the ellipsoid \\(x^2 + 2y^2 + 3z^2 = 1\\) attains its maximum."\n        }\n    ],\n    "conclusion": "The points (1, 0, 0) and (-1, 0, 0) on the ellipsoid \\(x^2 + 2y^2 + 3z^2 = 1\\) have the largest distance from the origin.",\n    "status": "proved",\n    "proof": {\n        "type": "proof",\n        "steps": [\n            {\n                "type": "define",\n                "statement": "Define the functions \\(g: \\mathbb{R}^3 \\to \\mathbb{R}\\) such that \\(g(x, y, z) = x^2 + 2y^2 + 3z^2\\) and \\(f: \\mathbb{R}^3 \\to \\mathbb{R}\\) such that \\(f(x, y, z) = x^2 + y^2 + z^2\\).",\n                "term": ["g(x,y,z)", "f(x,y,z)"]\n            },\n            {\n                "type": "remark",\n                "statement": "Note that given \\((x, y, z)\\), \\(f\\) returns the square of the point\'s distance \\(d\\) from the origin. Maximizing \\(d\\) is the same as maximizing \\(d^2\\) (since \\(d \\geq 0\\))."\n            },\n            {\n                "type": "remark",\n                "statement": "The problem is to maximize \\(f\\) under the constraint \\(g(x, y, z) = 1\\)."\n            },\n            {\n                "type": "assert",\n                "claim": "At the restricted extremum of \\(f\\), \\(\\nabla g \\cdot \\nabla f = 0\\) (Lagrange multipliers)."\n            },\n            {\n                "type": "assert",\n                "claim": "The gradients are given by \\(\\nabla g = \\begin{pmatrix} 2x \\\\ 4y \\\\ 6z \\end{pmatrix}\\) and \\(\\nabla f = \\begin{pmatrix} 2x \\\\ 2y \\\\ 2z \\end{pmatrix}\\)."\n            },\n            {\n                "type": "assert",\n                "claim": "\\(\\begin{pmatrix} 2x \\\\ 4y \\\\ 6z \\end{pmatrix} = \\lambda \\begin{pmatrix} 2x \\\\ 2y \\\\ 2z \\end{pmatrix}\\)."\n            },\n            {\n                "type": "assert",\n                "claim": "\\(\\begin{aligned} 2x &= \\lambda 2x\\\\ 4y &= \\lambda 2y\\\\ 6z &= \\lambda 2z \\end{aligned}\\)."\n            },\n            {\n                "type": "cases",\n                "on": "values of \\(\\lambda\\)",\n                "split-kind": "condition",\n                "proof-cases": [\n                    {\n                        "type": "case",\n                        "condition": "\\(\\lambda = 1\\) and \\(y = z = 0\\)",\n                        "proof": {\n                            "type": "proof",\n                            "steps": [\n                                {\n                                    "type": "assert",\n                                    "claim": "Substituting \\(y = z = 0\\) in \\(g(x, y, z) = 1\\), we get \\(x^2 = 1\\) (\\(x = 1\\) or \\(x = -1\\))."\n                                },\n                                {\n                                    "type": "assert",\n                                    "claim": "Substituting \\(x = \\pm 1\\) and \\(y = z = 0\\) in \\(f(x, y, z)\\), we get \\(f(1, 0, 0) = f(-1, 0, 0) = 1\\)."\n                                }\n                            ]\n                        }\n                    },\n                    {\n                        "type": "case",\n                        "condition": "\\(\\lambda = 2\\) and \\(x = z = 0\\)",\n                        "proof": {\n                            "type": "proof",\n                            "steps": [\n                                {\n                                    "type": "assert",\n                                    "claim": "Substituting \\(x = z = 0\\) in \\(g(x, y, z) = 1\\), we get \\(y^2 = \\frac{1}{2}\\) (\\(y = \\pm \\frac{1}{\\sqrt{2}}\\))."\n                                },\n                                {\n                                    "type": "assert",\n                                    "claim": "Substituting \\(y = \\pm \\frac{1}{\\sqrt{2}}\\) and \\(x = z = 0\\) in \\(f(x, y, z)\\), we get \\(f(0, \\frac{1}{\\sqrt{2}}, 0) = f(0, -\\frac{1}{\\sqrt{2}}, 0) = \\frac{1}{2}\\)."\n                                }\n                            ]\n                        }\n                    },\n                    {\n                        "type": "case",\n                        "condition": "\\(\\lambda = 3\\) and \\(x = y = 0\\)",\n                        "proof": {\n                            "type": "proof",\n                            "steps": [\n                                {\n                                    "type": "assert",\n                                    "claim": "Substituting \\(x = y = 0\\) in \\(g(x, y, z) = 1\\), we get \\(3z^2 = 1\\) (\\(z = \\pm \\frac{1}{\\sqrt{3}}\\))."\n                                },\n                                {\n                                    "type": "assert",\n                                    "claim": "Substituting \\(z = \\pm \\frac{1}{\\sqrt{3}}\\) and \\(x = y = 0\\) in \\(f(x, y, z)\\), we get \\(f(0, 0, \\frac{1}{\\sqrt{3}}) = f(0, 0, -\\frac{1}{\\sqrt{3}}) = \\frac{1}{3}\\)."\n                                }\n                            ]\n                        }\n                    }\n                ]\n            },\n            {\n                "type": "conclude",\n                "statement": "\\(\\therefore f\\) is maximum in \\textbf{case 1}."\n            },\n            {\n                "type": "conclude",\n                "statement": "\\(\\therefore\\) the points \\((1, 0, 0)\\) and \\((-1, 0, 0)\\) have the largest distance from the origin, given by \\(d = \\sqrt{1} = 1\\)."\n            }\n        ]\n    }\n}\n```', '```json\n{\n  "type": "theorem",\n  "name": "Maximum Distance on Ellipsoid",\n  "hypothesis": [\n    {\n      "type": "assume",\n      "statement": "Any continuous function on the ellipsoid x^2 + 2y^2 + 3z^2 = 1 attains its maximum."\n    }\n  ],\n  "conclusion": "The points (1, 0, 0) and (-1, 0, 0) on the ellipsoid x^2 + 2y^2 + 3z^2 = 1 have the largest distance from the origin.",\n  "status": "proved",\n  "proof": {\n    "type": "proof",\n    "steps": [\n      {\n        "type": "define",\n        "term": "g",\n        "statement": "g(x, y, z) = x^2 + 2y^2 + 3z^2"\n      },\n      {\n        "type": "define",\n        "term": "f",\n        "statement": "f(x, y, z) = x^2 + y^2 + z^2"\n      },\n      {\n        "type": "remark",\n        "statement": "f returns the square of the distance from the origin."\n      },\n      {\n        "type": "assert",\n        "claim": "Maximizing the distance d is equivalent to maximizing d^2.",\n        "proof-method": "d ≥ 0"\n      },\n      {\n        "type": "assert",\n        "claim": "The problem reduces to maximizing f(x, y, z) under the constraint g(x, y, z) = 1.",\n        "proof-method": "constraint optimization"\n      },\n      {\n        "type": "assert",\n        "claim": "At the extremum, ∇g · ∇f must hold (Lagrange multipliers)."\n      },\n      {\n        "type": "assert",\n        "claim": "The gradients are ∇g(x, y, z) = (2x, 4y, 6z) and ∇f(x, y, z) = (2x, 2y, 2z)."\n      },\n      {\n        "type": "assert",\n        "claim": "2x = λ2x, 4y = λ2y, 6z = λ2z.",\n        "deduced_from": [\n          "∇g = λ∇f"\n        ]\n      },\n      {\n        "type": "cases",\n        "on": "λ",\n        "split-kind": "condition",\n        "proof-cases": [\n          {\n            "type": "case",\n            "condition": "λ = 1 and y = z = 0",\n            "proof": {\n              "type": "proof",\n              "steps": [\n                {\n                  "type": "assert",\n                  "claim": "x^2 = 1, so x = 1 or x = -1.",\n                  "deduced_from": [\n                    "g(x, y, z) = 1"\n                  ]\n                },\n                {\n                  "type": "assert",\n                  "claim": "f(1, 0, 0) = f(-1, 0, 0) = 1"\n                }\n              ]\n            }\n          },\n          {\n            "type": "case",\n            "condition": "λ = 2 and x = z = 0",\n            "proof": {\n              "type": "proof",\n              "steps": [\n                {\n                  "type": "assert",\n                  "claim": "y^2 = 1/4, so y = ±1/2.",\n                  "deduced_from": [\n                    "g(x, y, z) = 1"\n                  ]\n                },\n                {\n                  "type": "assert",\n                  "claim": "f(0, 1/2, 0) = f(0, -1/2, 0) = 1/4"\n                }\n              ]\n            }\n          },\n          {\n            "type": "case",\n            "condition": "λ = 3 and x = y = 0",\n            "proof": {\n              "type": "proof",\n              "steps": [\n                {\n                  "type": "assert",\n                  "claim": "3z^2 = 1, so z = ±1/√3.",\n                  "deduced_from": [\n                    "g(x, y, z) = 1"\n                  ]\n                },\n                {\n                  "type": "assert",\n                  "claim": "f(0, 0, 1/√3) = f(0, 0, -1/√3) = 1/3"\n                }\n              ]\n            }\n          }\n        ]\n      },\n      {\n        "type": "conclude",\n        "statement": "f is maximum in case ①. Therefore, the points (1, 0, 0) and (-1, 0, 0) have the largest distance from the origin, given by d = √1 = 1."\n      }\n    ]\n  }\n}\n```']