## Theorem: Prove that the points (1, 0, 0) and (-1, 0, 0) on the ellipsoid \( x^{2}+2 y^{2}+3 z^{2}=1 \) have the largest distance from the origin. You may assume that any continuous function on the ellipsoid attains its maximum.


## Proof: ['```json\n{\n  "type": "theorem",\n  "name": "Maximum Distance from Origin on Ellipsoid",\n  "hypothesis": [\n    {\n      "type": "assume",\n      "statement": "Any continuous function on the ellipsoid \\( x^2 + 2y^2 + 3z^2 = 1 \\) attains its maximum."\n    }\n  ],\n  "conclusion": "The points (1, 0, 0) and (-1, 0, 0) on the ellipsoid \\( x^2 + 2y^2 + 3z^2 = 1 \\) have the largest distance from the origin.",\n  "status": "proved",\n  "proof": {\n    "type": "proof",\n    "steps": [\n      {\n        "type": "let",\n        "variable": "f(x,y,z)",\n        "value": "x^2 + y^2 + z^2",\n        "kind": "function"\n      },\n      {\n        "type": "let",\n        "variable": "g(x,y,z)",\n        "value": "x^2 + 2y^2 + 3z^2 - 1",\n        "kind": "function"\n      },\n      {\n        "type": "assert",\n        "claim": "The problem of maximizing \\(f(x, y, z)\\) subject to \\(g(x, y, z) = 0\\) can be solved using Lagrange multipliers."\n      },\n      {\n        "type": "let",\n        "variable": "F(x,y,z)",\n        "value": "f(x,y,z) - \\lambda g(x,y,z)",\n        "kind": "function"\n      },\n      {\n        "type": "assert",\n        "claim": "At maxima or minima, \\(\\\\nabla F = 0\\)."\n      },\n      {\n        "type": "assert",\n        "claim": "\\\\( \\\\nabla((1 - \\\\lambda)x^2 + (1 - 2 \\\\lambda)y^2 + (1 - 3 \\\\lambda)z^2 + \\\\lambda) = 0 \\\\)",\n        "deduced_from": [\n          "\\\\( \\\\nabla F = 0 \\\\)"\n        ]\n      },\n      {\n        "type": "assert",\n        "claim": "\\\\( (1 - \\\\lambda) \\\\cdot 2x \\\\hat{i} + (1 - 2\\\\lambda) \\\\cdot 2y \\\\hat{j} + (1 - 3\\\\lambda) \\\\cdot 2z \\\\hat{k} = 0 \\\\)"\n      },\n      {\n        "type": "cases",\n        "on": "\\\\lambda",\n        "split-kind": "condition",\n        "proof-cases": [\n          {\n            "type": "case",\n            "condition": "\\\\lambda = 1",\n            "proof": {\n              "type": "proof",\n              "steps": [\n                {\n                  "type": "assert",\n                  "claim": "y_o = z_o = 0"\n                },\n                {\n                  "type": "assert",\n                  "claim": "x_o = \\\\pm 1"\n                },\n                {\n                  "type": "assert",\n                  "claim": "x_o^2 + y_o^2 + z_o^2 = 1"\n                }\n              ]\n            }\n          },\n          {\n            "type": "case",\n            "condition": "\\\\lambda = \\\\frac{1}{2}",\n            "proof": {\n              "type": "proof",\n              "steps": [\n                {\n                  "type": "assert",\n                  "claim": "x_o = z_o = 0"\n                },\n                {\n                  "type": "assert",\n                  "claim": "y_o = \\\\pm \\\\frac{1}{\\\\sqrt{2}}"\n                },\n                {\n                  "type": "assert",\n                  "claim": "x_o^2 + y_o^2 + z_o^2 = \\\\frac{1}{2}"\n                }\n              ]\n            }\n          },\n          {\n            "type": "case",\n            "condition": "\\\\lambda = \\\\frac{1}{3}",\n            "proof": {\n              "type": "proof",\n              "steps": [\n                {\n                  "type": "assert",\n                  "claim": "x_o = y_o = 0"\n                },\n                {\n                  "type": "assert",\n                  "claim": "z_o = \\\\pm \\\\frac{1}{\\\\sqrt{3}}"\n                },\n                {\n                  "type": "assert",\n                  "claim": "x_o^2 + y_o^2 + z_o^2 = \\\\frac{1}{3}"\n                }\n              ]\n            }\n          },\n          {\n            "type": "case",\n            "condition": "\\\\lambda = \\\\frac{1}{3}",\n            "proof": {\n              "type": "proof",\n              "steps": [\n                {\n                  "type": "assert",\n                  "claim": "x_o = y_o = z_o = 0"\n                },\n                {\n                  "type": "assert",\n                  "claim": "x_o^2 + y_o^2 + z_o^2 = 0"\n                }\n              ]\n            }\n          }\n        ]\n      },\n      {\n        "type": "conclude",\n        "statement": "The maximum value of \\( x_o^2 + y_o^2 + z_o^2 \\) occurs at the points (1, 0, 0) or (-1, 0, 0)."\n      }\n    ]\n  }\n}\n```', '```json\n{\n  "type": "theorem",\n  "name": "Maximal Distance on Ellipsoid",\n  "hypothesis": [\n    {\n      "type": "assume",\n      "statement": "x^2 + 2y^2 + 3z^2 = 1"\n    },\n    {\n      "type": "assume",\n      "statement": "Any continuous function on the ellipsoid attains its maximum."\n    }\n  ],\n  "conclusion": "The points (1, 0, 0) and (-1, 0, 0) on the ellipsoid x^2 + 2y^2 + 3z^2 = 1 have the largest distance from the origin.",\n  "status": "proved",\n  "proof": {\n    "type": "proof",\n    "steps": [\n      {\n        "type": "define",\n        "term": "f(x,y,z)",\n        "statement": "f(x,y,z) = x^2 + y^2 + z^2"\n      },\n      {\n        "type": "define",\n        "term": "g(x,y,z)",\n        "statement": "g(x,y,z) = x^2 + 2y^2 + 3z^2 - 1"\n      },\n      {\n        "type": "let",\n        "variable": "F(x,y,z)",\n        "value": "f - λg"\n      },\n      {\n        "type": "assert",\n        "claim": "∇F = 0 at maxima or minima",\n        "proof-method": "Using the concept of Lagrange multipliers"\n      },\n      {\n        "type": "assert",\n        "claim": "∇((1 - λ)x^2 + (1 - 2λ)y^2 + (1 - 3λ)z^2 + λ) = 0",\n        "deduced_from": ["∇F = 0"]\n      },\n      {\n        "type": "assert",\n        "claim": "(1 - λ)2x i + (1 - 2λ)2y j + (1 - 3λ)2z k = 0",\n        "deduced_from": ["∇((1 - λ)x^2 + (1 - 2λ)y^2 + (1 - 3λ)z^2 + λ) = 0"]\n      },\n      {\n        "type": "cases",\n        "on": "λ",\n        "split-kind": "condition",\n        "proof-cases": [\n          {\n            "type": "case",\n            "condition": "λ = 1",\n            "proof": {\n              "type": "proof",\n              "steps": [\n                {\n                  "type": "let",\n                  "variable": "y_o",\n                  "value": 0\n                },\n                {\n                  "type": "let",\n                  "variable": "z_o",\n                  "value": 0\n                },\n                {\n                  "type": "assert",\n                  "claim": "x_o = ±1",\n                  "deduced_from": ["x^2 + 2y^2 + 3z^2 = 1"]\n                },\n                {\n                  "type": "assert",\n                  "claim": "x_o^2 + y_o^2 + z_o^2 = 1"\n                }\n              ]\n            }\n          },\n          {\n            "type": "case",\n            "condition": "λ = 1/2",\n            "proof": {\n              "type": "proof",\n              "steps": [\n                {\n                  "type": "let",\n                  "variable": "x_o",\n                  "value": 0\n                },\n                {\n                  "type": "let",\n                  "variable": "z_o",\n                  "value": 0\n                },\n                {\n                  "type": "assert",\n                  "claim": "y_o = ± 1/√2",\n                  "deduced_from": ["x^2 + 2y^2 + 3z^2 = 1"]\n                },\n                {\n                  "type": "assert",\n                  "claim": "x_o^2 + y_o^2 + z_o^2 = 1/2"\n                }\n              ]\n            }\n          },\n          {\n            "type": "case",\n            "condition": "λ = 1/3",\n            "proof": {\n              "type": "proof",\n              "steps": [\n                {\n                  "type": "let",\n                  "variable": "x_o",\n                  "value": 0\n                },\n                {\n                  "type": "let",\n                  "variable": "y_o",\n                  "value": 0\n                },\n                {\n                  "type": "assert",\n                  "claim": "z_o = ± 1/√3",\n                  "deduced_from": ["x^2 + 2y^2 + 3z^2 = 1"]\n                },\n                {\n                  "type": "assert",\n                  "claim": "x_o^2 + y_o^2 + z_o^2 = 1/3"\n                }\n              ]\n            }\n          },\n          {\n            "type": "case",\n            "condition": "λ = 0",\n            "proof": {\n              "type": "proof",\n              "steps": [\n                {\n                  "type": "assert",\n                  "claim": "x_o = y_o = z_o = 0"\n                },\n                {\n                  "type": "assert",\n                  "claim": "x_o^2 + y_o^2 + z_o^2 = 0"\n                }\n              ]\n            }\n          }\n        ]\n      },\n      {\n        "type": "assert",\n        "claim": "The maximum value of x_o^2 + y_o^2 + z_o^2 is 1.",\n        "deduced_from": ["Cases"]\n      },\n      {\n        "type": "conclude",\n        "statement": "The points (1, 0, 0) and (-1, 0, 0) on the ellipsoid x^2 + 2y^2 + 3z^2 = 1 have the largest distance from the origin."\n      }\n    ]\n  }\n}\n```', '```json\n{\n  "type": "theorem",\n  "name": "Largest Distance from the Origin on Ellipsoid",\n  "hypothesis": [\n    {\n      "type": "assume",\n      "statement": "x^2 + 2y^2 + 3z^2 = 1"\n    }\n  ],\n  "conclusion": "The points (1, 0, 0) and (-1, 0, 0) on the ellipsoid x^2 + 2y^2 + 3z^2 = 1 have the largest distance from the origin.",\n  "status": "proved",\n  "proof": {\n    "type": "proof",\n    "steps": [\n      {\n        "type": "let",\n        "variable": "f(x, y, z)",\n        "value": "x^2 + y^2 + z^2",\n        "kind": "function"\n      },\n      {\n        "type": "let",\n        "variable": "g(x, y, z)",\n        "value": "x^2 + 2y^2 + 3z^2 - 1",\n        "kind": "function"\n      },\n      {\n        "type": "assume",\n        "statement": "We use the method of Lagrange multipliers."\n      },\n      {\n        "type": "let",\n        "variable": "F(x, y, z)",\n        "value": "f - λg",\n        "kind": "function"\n      },\n      {\n        "type": "assert",\n        "claim": "∇F = 0 at maxima or minima",\n        "proof-method": "By the method of Lagrange multipliers"\n      },\n      {\n        "type": "assert",\n        "claim": "∇((1 - λ)x^2 + (1 - 2λ)y^2 + (1 - 3λ)z^2 + λ) = 0",\n        "deduced_from": ["∇F = 0"],\n        "proof-method": "By calculating the gradient"\n      },\n      {\n        "type": "assert",\n        "claim": "(1 - λ)2x i + (1 - 2λ)2y j + (1 - 3λ)2z k = 0",\n        "deduced_from": ["∇((1 - λ)x^2 + (1 - 2λ)y^2 + (1 - 3λ)z^2 + λ) = 0"],\n        "proof-method": "By equating the gradient to zero"\n      },\n      {\n        "type": "cases",\n        "on": "λ",\n        "split-kind": "condition",\n        "proof-cases": [\n          {\n            "type": "case",\n            "condition": "λ = 1",\n            "proof": {\n              "type": "proof",\n              "steps": [\n                {\n                  "type": "assert",\n                  "claim": "y = 0 and z = 0",\n                  "proof-method": "From the equation (1 - λ)2x = 0, (1 - 2λ)2y = 0, (1 - 3λ)2z = 0"\n                },\n                {\n                  "type": "assert",\n                  "claim": "x = ±1",\n                  "proof-method": "Substitute in the constraint equation x^2 + 2y^2 + 3z^2 = 1"\n                },\n                {\n                  "type": "assert",\n                  "claim": "x^2 + y^2 + z^2 = 1",\n                  "proof-method": "Substitute the values x = ±1, y = 0, z = 0"\n                }\n              ]\n            }\n          },\n          {\n            "type": "case",\n            "condition": "λ = 1/2",\n            "proof": {\n              "type": "proof",\n              "steps": [\n                {\n                  "type": "assert",\n                  "claim": "x = 0 and z = 0",\n                  "proof-method": "From the equation (1 - λ)2x = 0, (1 - 2λ)2y = 0, (1 - 3λ)2z = 0"\n                },\n                {\n                  "type": "assert",\n                  "claim": "y = ±1/√2",\n                  "proof-method": "Substitute in the constraint equation x^2 + 2y^2 + 3z^2 = 1"\n                },\n                {\n                  "type": "assert",\n                  "claim": "x^2 + y^2 + z^2 = 1/2",\n                  "proof-method": "Substitute the values x = 0, y = ±1/√2, z = 0"\n                }\n              ]\n            }\n          },\n          {\n            "type": "case",\n            "condition": "λ = 1/3",\n            "proof": {\n              "type": "proof",\n              "steps": [\n                {\n                  "type": "assert",\n                  "claim": "x = 0 and y = 0",\n                  "proof-method": "From the equation (1 - λ)2x = 0, (1 - 2λ)2y = 0, (1 - 3λ)2z = 0"\n                },\n                {\n                  "type": "assert",\n                  "claim": "z = ±1/√3",\n                  "proof-method": "Substitute in the constraint equation x^2 + 2y^2 + 3z^2 = 1"\n                },\n                {\n                  "type": "assert",\n                  "claim": "x^2 + y^2 + z^2 = 1/3",\n                  "proof-method": "Substitute the values x = 0, y = 0, z = ±1/√3"\n                }\n              ]\n            }\n          },\n          {\n            "type": "case",\n            "condition": "λ = 0",\n            "proof": {\n              "type": "proof",\n              "steps": [\n                {\n                  "type": "assert",\n                  "claim": "x = 0, y = 0, z = 0",\n                  "proof-method": "From the equation (1 - λ)2x = 0, (1 - 2λ)2y = 0, (1 - 3λ)2z = 0"\n                },\n                {\n                  "type": "assert",\n                  "claim": "x^2 + y^2 + z^2 = 0",\n                  "proof-method": "Substitute the values x = 0, y = 0, z = 0"\n                }\n              ]\n            }\n          }\n        ]\n      },\n      {\n        "type": "assert",\n        "claim": "The maximum value of x^2 + y^2 + z^2 is 1",\n        "deduced_from": [\n          "Cases analysis shows that 1 is the maximum value of x^2 + y^2 + z^2 on the ellipsoid"\n        ]\n      },\n      {\n        "type": "conclude",\n        "statement": "The maximum value of x^2 + y^2 + z^2 is attained at the points (1, 0, 0) and (-1, 0, 0)."\n      }\n    ]\n  }\n}\n```']