## Theorem: Consider the linear differential equation \( \dot{x}=y \) and \( \dot{y}=x). Prove that the origin is saddle.



## Proof: The system is given by 
$\dot{X} = \begin{bmatrix} 0 & 1 \\ 1 & 0 \end{bmatrix} \begin{bmatrix} x \\ y \end{bmatrix}$. 

First, we find the eigenvalues of the matrix $A = \begin{bmatrix} 0 & 1 \\ 1 & 0 \end{bmatrix}$.  The characteristic equation is 
$|A - \lambda I| = 0$,
which simplifies to 
$\begin{vmatrix} -\lambda & 1 \\ 1 & -\lambda \end{vmatrix} = 0$. 
This gives us $\lambda^2 - 1 = 0$,
so $\lambda = \pm 1$. 

For $\lambda = 1$, we solve the system 
$\begin{bmatrix} -1 & 1 \\ 1 & -1 \end{bmatrix} \begin{bmatrix} x \\ y \end{bmatrix} = \begin{bmatrix} 0 \\ 0 \end{bmatrix}$. 
This gives us $-x + y = 0$,
or $x = y$. 
Hence, a corresponding eigenvector is $\begin{bmatrix} 1 \\ 1 \end{bmatrix}$. 

For $\lambda = -1$, we solve the system 
$\begin{bmatrix} 1 & 1 \\ 1 & 1 \end{bmatrix} \begin{bmatrix} x \\ y \end{bmatrix} = \begin{bmatrix} 0 \\ 0 \end{bmatrix}$. 
This gives us $x = -y$. 
Hence, a corresponding eigenvector is $\begin{bmatrix} -1 \\ 1 \end{bmatrix}$. 

Therefore, the general solution is 
$X(t) = \alpha X_1(t) + \beta X_2(t) = \alpha \begin{bmatrix} 1 \\ 1 \end{bmatrix} e^t + \beta \begin{bmatrix} -1 \\ 1 \end{bmatrix} e^{-t}$. 

For $t \to \infty$, $X(t) \approx \alpha X_1(t)$. 
For $t \to -\infty$, $X(t) \approx \beta X_2(t)$. 

Clearly, the origin is a saddle point due to the intersection of the stable and unstable lines. 

$(1, 1)$ and $(1, -1)$ were chosen as sample vectors along the eigenvector lines. 

$\alpha, \beta \in \mathbb{R}$. 
