## Theorem: Consider the linear differential equation \( \dot{x}=y \) and \( \dot{y}=x). Prove that the origin is saddle.



## Proof: 5. a) $\dot{x} = y$ & $\dot{y} = x$ 
$\implies \frac{d}{dt} \begin{bmatrix}
x \\ 
y
\end{bmatrix} = \begin{bmatrix}
0 & 1 \\ 
1 & 0
\end{bmatrix} \begin{bmatrix}
x \\ 
y
\end{bmatrix}$
$\implies \dot{v} = Av$ where $A = \begin{bmatrix}
0 & 1 \\ 
1 & 0
\end{bmatrix}$
characteristic equation of $A$ is 
$\lambda^{2} - 1 = 0$
$\implies \lambda_{1} = 1$ & $\lambda_{2} = -1$
To find the eigen vectors
$Av_{1} = \begin{bmatrix}
0 & 1 \\ 
1 & 0
\end{bmatrix} \begin{bmatrix}
x_{1} \\ 
y_{1}
\end{bmatrix} = \begin{bmatrix}
x_{1} \\ 
y_{1}
\end{bmatrix}$ 
$\implies y_{1} = x_{1}$ & $x_{1} = y_{1}$, 
i.e. $v_{1} = \begin{pmatrix}
1 \\ 
1
\end{pmatrix}$
$Av_{2} = \begin{bmatrix}
0 & 1 \\ 
1 & 0
\end{bmatrix} \begin{bmatrix}
x_{2} \\ 
y_{2}
\end{bmatrix} = -\begin{bmatrix}
x_{2} \\ 
y_{2}
\end{bmatrix}$
$\implies y_{2} = -x_{2}$ & $x_{2} = -y_{2}$
$\implies v_{2} = \begin{pmatrix}
1 \\ 
-1
\end{pmatrix}$
... equation becomes
$\frac{d}{dt} \begin{bmatrix}
x \\ 
y
\end{bmatrix} = \begin{bmatrix}
0 & 1 \\ 
1 & 4
\end{bmatrix} \begin{bmatrix}
x \\ 
y
\end{bmatrix}$ where $\begin{bmatrix}
x \\ 
y
\end{bmatrix} \equiv x(c_{1}, 1) + y(c_{1}, -1)$
... on solving,
$\frac{dx}{dt} = x$ $\implies x = c_{1}e^{t}$
& $\frac{dy}{dt} = -y$ $\implies y = (c_{2} e^{-t}$
$\implies xy = c_{1}c_{2} = k$ (hyperbola)
... the "trajectory" would be a saddle with the axes along $(1, 1)$ & $(1, -1)$

---

We have that $\dot{x} = y$ and $\dot{y} = x$.  This implies that 
$$
\frac{d}{dt} \begin{bmatrix}
x \\ 
y
\end{bmatrix} = \begin{bmatrix}
0 & 1 \\ 
1 & 0
\end{bmatrix} \begin{bmatrix}
x \\ 
y
\end{bmatrix}.
$$
Thus we have $\dot{v} = Av$ where $A = \begin{bmatrix}
0 & 1 \\ 
1 & 0
\end{bmatrix}$.  The characteristic equation of $A$ is  $\lambda^{2} - 1 = 0$, so $\lambda_{1} = 1$ and  $\lambda_{2} = -1$.  To find the eigenvectors, we compute
$$
Av_{1} = \begin{bmatrix}
0 & 1 \\ 
1 & 0
\end{bmatrix} \begin{bmatrix}
x_{1} \\ 
y_{1}
\end{bmatrix} = \begin{bmatrix}
x_{1} \\ 
y_{1}
\end{bmatrix}.
$$
Thus $y_{1} = x_{1}$ and $x_{1} = y_{1}$, so $v_{1} = \begin{pmatrix}
1 \\ 
1
\end{pmatrix}$.
Similarly, 
$$
Av_{2} = \begin{bmatrix}
0 & 1 \\ 
1 & 0
\end{bmatrix} \begin{bmatrix}
x_{2} \\ 
y_{2}
\end{bmatrix} = -\begin{bmatrix}
x_{2} \\ 
y_{2}
\end{bmatrix}.
$$
Then $y_{2} = -x_{2}$ and $x_{2} = -y_{2}$, so
$\implies v_{2} = \begin{pmatrix}
1 \\ 
-1
\end{pmatrix}$.
Therefore the equation becomes
$$
\frac{d}{dt} \begin{bmatrix}
x \\ 
y
\end{bmatrix} = \begin{bmatrix}
0 & 1 \\ 
1 & 4
\end{bmatrix} \begin{bmatrix}
x \\ 
y
\end{bmatrix},
$$
where $\begin{bmatrix}
x \\ 
y
\end{bmatrix} \equiv x(c_{1}, 1) + y(c_{1}, -1)$.  Solving, we see that $\frac{dx}{dt} = x$, which implies $x = c_{1}e^{t}$.
Also, $\frac{dy}{dt} = -y$, so $y = (c_{2} e^{-t}$.  Thus $xy = c_{1}c_{2} = k$, which is a hyperbola.  Therefore the trajectory would be a saddle with the axes along $(1, 1)$ & $(1, -1)$.
