## Theorem: Consider the linear differential equation \( \dot{x}=y \) and \( \dot{y}=x). Prove that the origin is saddle.



## Proof: 5. (a) $\dot x = y$, $\dot y = x$

$A\begin{bmatrix} \dot x \\ \dot y \end{bmatrix} = \begin{bmatrix} y \\ x \end{bmatrix}$

$\implies A\begin{bmatrix} x \\ y \end{bmatrix} = \begin{bmatrix} y \\ x \end{bmatrix}$

$\implies \begin{bmatrix} 0 & 1 \\ 1 & 0 \end{bmatrix} \begin{bmatrix} y \\ x \end{bmatrix} = \begin{bmatrix} y \\ x \end{bmatrix}$

Thus $A = \begin{bmatrix} 0 & 1 \\ 1 & 0 \end{bmatrix}$

Let us find the eigen values

$\det(A-\lambda I) = 0$

$\det \begin{bmatrix} -\lambda & 1 \\ 1 & -\lambda \end{bmatrix} + \begin{bmatrix} - \lambda & 0 \\ 0 & - \lambda \end{bmatrix} = 0$

$\det \begin{bmatrix} -\lambda & 1 \\ 1 & - \lambda \end{bmatrix} = 0$

$\lambda^2 - 1 = 0$

$\boxed{\lambda = \pm 1}$

we calculate

when $\lambda_1 = 1$

$(A - I) = \begin{bmatrix} -1 & 1 \\ 1 & -1 \end{bmatrix}$

$\begin{bmatrix} -1 & 1 \\ 1 & -1 \end{bmatrix} \begin{bmatrix} x \\ y \end{bmatrix} = \begin{bmatrix} 0 \\ 0 \end{bmatrix}$

$-x + y = 0$

$x-y = 0$

$\boxed{x = y}$

Let us take eigen vector as $v_1 = \begin{bmatrix} 1 \\ 1 \end{bmatrix}$

when $\lambda_2 = -1$

$(A+I) = \begin{bmatrix} 1 & 1 \\ 1 & 1 \end{bmatrix}$

$\begin{bmatrix} 1 & 1 \\ 1 & 1 \end{bmatrix} \begin{bmatrix} x \\ y \end{bmatrix} = \begin{bmatrix} 0 \\ 0 \end{bmatrix}$

$x+y = 0$

$\boxed{-x = +y}$

take eigen vector example as $v_2 = \begin{bmatrix} 1 \\ -1 \end{bmatrix}$

Thus $x(t) = \alpha e^t \begin{bmatrix} 1 \\ 1 \end{bmatrix} + \beta e^{-t} \begin{bmatrix} 1 \\ -1 \end{bmatrix}$

This has a saddle  origin

$y = x$



**Cleaned-up Proof:**

We are given the system of differential equations $\dot{x} = y$ and $\dot{y} = x$. We can rewrite this system in matrix form as $A \begin{bmatrix} x \\ y \end{bmatrix} = \begin{bmatrix} y \\ x \end{bmatrix}$, where $A = \begin{bmatrix} 0 & 1 \\ 1 & 0 \end{bmatrix}$.

To find the eigenvalues of $A$, we solve the characteristic equation $\det(A - \lambda I) = 0$. This gives us $\lambda^2 - 1 = 0$, which has solutions $\lambda = \pm 1$.

For $\lambda_1 = 1$, we solve the equation $(A - I) \begin{bmatrix} x \\ y \end{bmatrix} = \begin{bmatrix} 0 \\ 0 \end{bmatrix}$. This gives us the equation $x = y$. We can take the eigenvector $v_1 = \begin{bmatrix} 1 \\ 1 \end{bmatrix}$.

For $\lambda_2 = -1$, we solve the equation $(A + I) \begin{bmatrix} x \\ y \end{bmatrix} = \begin{bmatrix} 0 \\ 0 \end{bmatrix}$. This gives us the equation $-x = y$. We can take the eigenvector $v_2 = \begin{bmatrix} 1 \\ -1 \end{bmatrix}$.

Thus, the general solution to the system of differential equations is given by $x(t) = \alpha e^t \begin{bmatrix} 1 \\ 1 \end{bmatrix} + \beta e^{-t} \begin{bmatrix} 1 \\ -1 \end{bmatrix}$, where $\alpha$ and $\beta$ are constants. This solution corresponds to a saddle point at the origin. 
