## Theorem: For the linear differential equation \( \dot{x}=y \) and \( \dot{y}=-x-y). Prove that the origin is circulation.


## Proof: The given matrix is  
$\begin{pmatrix} \frac{1 - \sqrt{3}i}{2} & 1 \\ -1 & \frac{-1 - \sqrt{3}i}{2}  \end{pmatrix}$.

We have 
$\begin{pmatrix} \frac{1 - \sqrt{3}i}{2} & 1 \\ -1 & \frac{-1 - \sqrt{3}i}{2}  \end{pmatrix}  \begin{pmatrix} a \\ b \end{pmatrix} = \begin{pmatrix} 0 \\ 0 \end{pmatrix}$.
Then 
$-a \begin{pmatrix} \frac{1 - \sqrt{3}i}{2}  \\ 2  \end{pmatrix} = ab$.
So $a = -b \begin{pmatrix} \frac{1 + \sqrt{3}i}{2} \end{pmatrix}$. This implies that 
$b = \frac{-2a(1 - \sqrt{3}i)}{(1 + \sqrt{3}i)(1 - \sqrt{3}i)} = \frac{-a (1 - \sqrt{3}i)}{2}$.

The eigenvector for $\lambda_1$ is $\begin{pmatrix} \frac{-\sqrt{3}i - 1}{2} \\ 1 \end{pmatrix} = V_1$.

The eigenvector for $\lambda_2$ is $\begin{pmatrix} \frac{1 + \sqrt{3}i}{2} \\ -1 \end{pmatrix}$. We have $\begin{pmatrix} \frac{1 + \sqrt{3}i}{2} & 1 \\ -1 & \frac{-1 + \sqrt{3}i}{2}  \end{pmatrix} \begin{pmatrix} a \\ b \end{pmatrix} = \begin{pmatrix} 0 \\ 0 \end{pmatrix}$.
Then $a \begin{pmatrix} \frac{1 + \sqrt{3}i}{2} \\ 2  \end{pmatrix} = b$.
So $-a = b  \begin{pmatrix} \frac{\sqrt{3}i - 1}{2}  \end{pmatrix}$.
This implies that $a  \begin{pmatrix} \frac{1 + \sqrt{3}i}{2}  \end{pmatrix} = b$.

Therefore, $V_2 = \begin{pmatrix} \frac{1 + \sqrt{3}i}{2} \\ 1 \end{pmatrix}$.
