## Theorem: For the linear differential equation \( \dot{x}=y \) and \( \dot{y}=-x-y). Prove that the origin is circulation.


## Proof: **(4)** $\dot{x} = y$
$\dot{y} = -x - y$
$\begin{bmatrix} \dot{x} \\ \dot{y} \end{bmatrix} = \begin{bmatrix} 0 & 1 \\ -1 & -1 \end{bmatrix} \begin{bmatrix} x \\ y \end{bmatrix}$

$X' = AX$

$|A - \lambda I| = \begin{vmatrix} -\lambda & 1 \\ -1 & -1-\lambda \end{vmatrix} = 0$

$\lambda(1+\lambda) + 1 = 0$
$\implies \lambda^2 + \lambda + 1 = 0$
$\lambda = \dfrac{-1 \pm \sqrt{1-4}}{2}$

$= \dfrac{-1 \pm i\sqrt{3}}{2} = \dfrac{-1}{2} \pm \dfrac{\sqrt{3}i}{2}$
The imaginary part of $\lambda$ ($\pm \frac{\sqrt{3}i}{2}$) gives a circulation. 
$X(t) = V_1$

The real part of $\lambda$ $(= -\frac{1}{2})$, when superposed on the circulation, gives a spiralling decay with time.

$X(t) = \alpha e^{-\frac{t}{2}}F(t)$ / $F(t)$ is the circulation-equivalent part of $X(t)$.

As $t\to \infty$
$X(t) \to 0$.

So, the origin acts as a SPIRAL SINK. 

[Image of a spiral converging to the origin]

Sense of spiral depends on the sign of parameters.
