## Theorem: For the linear differential equation \( \dot{x}=y \) and \( \dot{y}=-x-y). Prove that the origin is circulation.


## Proof: (d) $\dot{x} = y$ $\dot{y} = -x-y$

$A = \begin{bmatrix} 0 & 1 \\ -1 & -1 \end{bmatrix}$ $X' = AX$

Characteristic equation : $(\lambda)(\lambda + 1) - (-1)(1) = 0$
$\lambda^2 + \lambda + 1 = 0$
$\lambda = \dfrac{-1 \pm \sqrt{1-4}}{2} = \dfrac{-1}{2} \pm i \dfrac{\sqrt{3}}{2}$

For $\lambda = \dfrac{-1}{2} + i\dfrac{\sqrt{3}}{2}$
$(A - \lambda I)\begin{bmatrix} x \\ y \end{bmatrix} = 0$
$\begin{bmatrix} -\frac{1}{2} - i \frac{\sqrt{3}}{2} & 1 \\ -1 & -\frac{1}{2} - i \frac{\sqrt{3}}{2} \end{bmatrix} \begin{bmatrix} x \\ y \end{bmatrix} = 0$

$(\frac{-1}{2} - i \frac{\sqrt{3}}{2})x + y = 0$
$y = (\frac{1}{2} + i \frac{\sqrt{3}}{2})x$

$V_2 = \begin{bmatrix} 1 \\ \frac{1}{2} + i \frac{\sqrt{3}}{2} \end{bmatrix}$ is an eigenvector.

Solution: 
$X(t) = \alpha e^{\begin{bmatrix} 1 \\ -1 + i \frac{\sqrt{3}}{2} \end{bmatrix}t}$

$X(t) = \alpha e^{\frac{-t}{2} } \begin{bmatrix} 2\cos(\frac{\sqrt{3}}{2}t) + 2i\sin(\frac{\sqrt{3}}{2}t) \\ [\cos(\frac{\sqrt{3}}{2}t)-i\sin(\frac{\sqrt{3}}{2}t)] + i[\cos(\frac{\sqrt{3}}{2}t) - \sin(\frac{\sqrt{3}}{2}t)]\end{bmatrix}$

$X(t) = \alpha e^{\frac{-t}{2}} \begin{bmatrix} 2 \cos(\frac{\sqrt{3}}{2}t) \\ \frac{-1}{2} \cos(\frac{\sqrt{3}}{2}t) - \frac{\sqrt{3}}{2}\sin(\frac{\sqrt{3}}{2}t)\end{bmatrix}$

$Re \ X(t) = \alpha e^{\frac{-t}{2}} \begin{bmatrix} \cos(\frac{\sqrt{3}}{2}t) \\ \frac{-1}{2}\cos(\frac{\sqrt{3}}{2}t) - \frac{\sqrt{3}}{2} \sin(\frac{\sqrt{3}}{2}t)\end{bmatrix}$

$Im \ X(t) = \alpha e^{\frac{-t}{2}} \begin{bmatrix} \sin(\frac{\sqrt{3}}{2}t) \\ \frac{\sqrt{3}}{2} \cos(\frac{\sqrt{3}}{2}t) - \frac{1}{2}\sin(\frac{\sqrt{3}}{2}t)\end{bmatrix}$

These are solutions to $X' = AX$
General Solution :
$X(t) = \alpha e^{\frac{-t}{2}} \begin{bmatrix} 2\cos(\frac{\sqrt{3}}{2}t) \\ \frac{-1}{2}\cos(\frac{\sqrt{3}}{2}t) - \frac{\sqrt{3}}{2} \sin(\frac{\sqrt{3}}{2}t)\end{bmatrix} + \beta e^{\frac{-t}{2}} \begin{bmatrix} 2\sin(\frac{\sqrt{3}}{2}t) \\ \frac{\sqrt{3}}{2} \cos(\frac{\sqrt{3}}{2}t) - \frac{1}{2}\sin(\frac{\sqrt{3}}{2}t)\end{bmatrix}$

This is a spiral sink as it has a negative exponential and spirals around due to the sinusoidal functions.

---

We are given that $\dot{x} = y$ and $\dot{y} = -x-y$.  Let $A = \begin{bmatrix} 0 & 1 \\ -1 & -1 \end{bmatrix}$.  Then we can write $X' = AX$.

The characteristic equation is $(\lambda)(\lambda + 1) - (-1)(1) = 0$, which simplifies to $\lambda^2 + \lambda + 1 = 0$.  Solving for $\lambda$, we get $\lambda = \dfrac{-1 \pm \sqrt{1-4}}{2} = \dfrac{-1}{2} \pm i \dfrac{\sqrt{3}}{2}$.

Now consider the case where $\lambda = \dfrac{-1}{2} + i\dfrac{\sqrt{3}}{2}$.  We want to find the eigenvectors of $(A - \lambda I)$, so we solve  $(A - \lambda I)\begin{bmatrix} x \\ y \end{bmatrix} = 0$.  This gives us 
$\begin{bmatrix} -\frac{1}{2} - i \frac{\sqrt{3}}{2} & 1 \\ -1 & -\frac{1}{2} - i \frac{\sqrt{3}}{2} \end{bmatrix} \begin{bmatrix} x \\ y \end{bmatrix} = 0$, which simplifies to $(\frac{-1}{2} - i \frac{\sqrt{3}}{2})x + y = 0$.  Solving for $y$, we get $y = (\frac{1}{2} + i \frac{\sqrt{3}}{2})x$.  Therefore, $V_2 = \begin{bmatrix} 1 \\ \frac{1}{2} + i \frac{\sqrt{3}}{2} \end{bmatrix}$ is an eigenvector.

Thus, a solution is $X(t) = \alpha e^{\begin{bmatrix} 1 \\ -1 + i \frac{\sqrt{3}}{2} \end{bmatrix}t}$.  Expanding this, we get
$X(t) = \alpha e^{\frac{-t}{2} } \begin{bmatrix} 2\cos(\frac{\sqrt{3}}{2}t) + 2i\sin(\frac{\sqrt{3}}{2}t) \\ [\cos(\frac{\sqrt{3}}{2}t)-i\sin(\frac{\sqrt{3}}{2}t)] + i[\cos(\frac{\sqrt{3}}{2}t) - \sin(\frac{\sqrt{3}}{2}t)]\end{bmatrix}$.

This simplifies to $X(t) = \alpha e^{\frac{-t}{2}} \begin{bmatrix} 2 \cos(\frac{\sqrt{3}}{2}t) \\ \frac{-1}{2} \cos(\frac{\sqrt{3}}{2}t) - \frac{\sqrt{3}}{2}\sin(\frac{\sqrt{3}}{2}t)\end{bmatrix}$.
Therefore, the real part of $X(t)$ is $Re \ X(t) = \alpha e^{\frac{-t}{2}} \begin{bmatrix} \cos(\frac{\sqrt{3}}{2}t) \\ \frac{-1}{2}\cos(\frac{\sqrt{3}}{2}t) - \frac{\sqrt{3}}{2} \sin(\frac{\sqrt{3}}{2}t)\end{bmatrix}$ and the imaginary part of $X(t)$ is $Im \ X(t) = \alpha e^{\frac{-t}{2}} \begin{bmatrix} \sin(\frac{\sqrt{3}}{2}t) \\ \frac{\sqrt{3}}{2} \cos(\frac{\sqrt{3}}{2}t) - \frac{1}{2}\sin(\frac{\sqrt{3}}{2}t)\end{bmatrix}$.

These are solutions to $X' = AX$.  Therefore, the general solution is 
$X(t) = \alpha e^{\frac{-t}{2}} \begin{bmatrix} 2\cos(\frac{\sqrt{3}}{2}t) \\ \frac{-1}{2}\cos(\frac{\sqrt{3}}{2}t) - \frac{\sqrt{3}}{2} \sin(\frac{\sqrt{3}}{2}t)\end{bmatrix} + \beta e^{\frac{-t}{2}} \begin{bmatrix} 2\sin(\frac{\sqrt{3}}{2}t) \\ \frac{\sqrt{3}}{2} \cos(\frac{\sqrt{3}}{2}t) - \frac{1}{2}\sin(\frac{\sqrt{3}}{2}t)\end{bmatrix}$.  This describes a spiral sink, as it has a negative exponential and spirals due to the sinusoidal functions.
