## Theorem: For the linear differential equation \( \dot{x}=y \) and \( \dot{y}=-x-y). Prove that the origin is circulation.


## Proof: The text in the image can be transcribed to the following:

$\vec{x} = \begin{bmatrix} x\\ y \end{bmatrix}$, $\vec{y} = \begin{bmatrix} 5\\ 5-x \end{bmatrix}$ when $A = \begin{pmatrix} 0 & 1\\ -1 & -1 \end{pmatrix}$ 

... $\vec{x}$ upon reduce $A$ then obtain an Ax ($\begin{pmatrix} 0 & 1\\ -1 & -1 \end{pmatrix} A$) $\begin{pmatrix} & & \\ 1 & & \\ \end{pmatrix}$ 

$\Rightarrow$ $\det = \begin{vmatrix} -\lambda & 1\\ -1 & -1-\lambda \end{vmatrix} = 0$

$\Rightarrow$ $-(1+\lambda)\lambda + 1 = 0$; $\frac{-1 \pm \sqrt{-3}}{2}$ $\therefore$ use 

also use eigen vector assessment tool Also $\lambda_{1} = \frac{-1 + i\sqrt{3}}{2}$, $\lambda_{2} = \frac{-1 - i\sqrt{3}}{2}$ 

... $A_{v_{1}} =$ ... 
$\Rightarrow$ $Av_{1} = \lambda v_{1} \Rightarrow$ $\begin{pmatrix}  & 1 & \\ -1 & -1 & \end{pmatrix}$ $\begin{pmatrix}  & & \\ 1 &  & \\  &  & \end{pmatrix}$ = $\begin{pmatrix}  & & \\ \sqrt{17} &  & \\  &  & \end{pmatrix}$

$\Rightarrow$ $Av_{1} = \frac{1}{2} \begin{pmatrix}  & & \\ \sqrt{1} &  & \\  &  & \end{pmatrix}$ - $\frac{\sqrt{3}}{2} \begin{pmatrix}  & & \\ \sqrt{2} &  & \\  &  & \end{pmatrix}$

$Av_{2} =$ -$\frac{1}{2}$ $\begin{pmatrix}  & & \\ 1 &  & \\  &  & \end{pmatrix}$ $1$ $\frac{\sqrt{3}}{2}$ $\begin{pmatrix}  & & \\ \sqrt{1} &  & \\  &  & \end{pmatrix}$

Cleaning up the text into full sentences, we have:

Let $\vec{x} = \begin{bmatrix} x\\ y \end{bmatrix}$ and  $\vec{y} = \begin{bmatrix} 5\\ 5-x \end{bmatrix}$ when $A = \begin{pmatrix} 0 & 1\\ -1 & -1 \end{pmatrix}$. 

... we reduce $A$ to obtain $\begin{pmatrix} 0 & 1\\ -1 & -1 \end{pmatrix} A$ $\begin{pmatrix} & & \\ 1 & & \\ \end{pmatrix}$.

This gives us the determinant $\det = \begin{vmatrix} -\lambda & 1\\ -1 & -1-\lambda \end{vmatrix} = 0$.

Hence $-(1+\lambda)\lambda + 1 = 0$, and we get $\frac{-1 \pm \sqrt{-3}}{2}$. Therefore, we use ...

We also use the eigenvector assessment tool. Also $\lambda_{1} = \frac{-1 + i\sqrt{3}}{2}$ and $\lambda_{2} = \frac{-1 - i\sqrt{3}}{2}$. 

... $A_{v_{1}} = $ ... 

This implies $Av_{1} = \lambda v_{1}$, which can be rewritten as $\begin{pmatrix}  & 1 & \\ -1 & -1 & \end{pmatrix}$ $\begin{pmatrix}  & & \\ 1 &  & \\  &  & \end{pmatrix}$ = $\begin{pmatrix}  & & \\ \sqrt{17} &  & \\  &  & \end{pmatrix}$.

This implies $Av_{1} = \frac{1}{2} \begin{pmatrix}  & & \\ \sqrt{1} &  & \\  &  & \end{pmatrix}$ - $\frac{\sqrt{3}}{2} \begin{pmatrix}  & & \\ \sqrt{2} &  & \\  &  & \end{pmatrix}$.

Finally, we have $Av_{2} =$ -$\frac{1}{2}$ $\begin{pmatrix}  & & \\ 1 &  & \\  &  & \end{pmatrix}$ $1$ $\frac{\sqrt{3}}{2}$ $\begin{pmatrix}  & & \\ \sqrt{1} &  & \\  &  & \end{pmatrix}$.

Please note that some parts of the original text are illegible or contain unclear notations, so the transcription might not be perfectly accurate. 
