## Theorem: For the linear differential equation \( \dot{x}=y \) and \( \dot{y}=-x-y). Prove that the origin is circulation.


## Proof: $\\~\\$
$\begin{pmatrix} \dot x \\ \dot y  \end{pmatrix} = \begin{pmatrix} 0 & 1 \\ -x & -y \end{pmatrix} = A \begin{pmatrix} x \\ y \end{pmatrix}$
$\\~\\$
$A = \begin{pmatrix} 0 & 1 \\ -1 & -1 \end{pmatrix}$
$\\~\\$

Eigenvalues for $A$ are 
$\\~\\$
$(-\lambda)(-\lambda -1)+1 = 0$
$\\~\\$
$\implies \lambda^2 + \lambda +1 = 0$
$\\~\\$
$\lambda_1 = \dfrac{-1+\sqrt{3}i}{2}  \quad ; \quad \lambda_2 = \dfrac{-1-\sqrt{3}i}{2}$
$\\~\\$

Eigenvectors corresponding to $\lambda_1$ is 
$\\~\\$
$\begin{pmatrix} \dfrac{-1-\sqrt{3}i}{2} & 1 \\ -1 & \dfrac{-1-\sqrt{3}i}{2}\end{pmatrix}\begin{pmatrix} a\\ b\end{pmatrix} = 0$
$\\~\\$
$-a(\dfrac{1-\sqrt{3}i}{2})-ab = 0$
$\\~\\$
$a = -b\dfrac{(1+\sqrt{3}i)}{2} \implies b = \dfrac{-a(1-\sqrt{3}i)}{(1+\sqrt{3}i)(1-\sqrt{3}i)} = \dfrac{-a(1-\sqrt{3}i)}{2}$
$\\~\\$
Eigen vector for $\lambda_1$ is $\begin{pmatrix} \sqrt{3}i - 1 \\ 2 \end{pmatrix} = v_1$
$\\~\\$
Eigen vector for $\lambda_2$ is 
$\\~\\$
$\begin{pmatrix} \dfrac{1+\sqrt{3}i}{2} & 1 \\ -1 &  \dfrac{-1+\sqrt{3}i}{2}\end{pmatrix}\begin{pmatrix} a\\ b\end{pmatrix} = \begin{pmatrix} 0 \\ 0 \end{pmatrix}$
$\\~\\$
$a(\dfrac{1+\sqrt{3}i}{2}) = b  \quad ; \quad -a = b (\dfrac{\sqrt{3}i - 1}{2})$
$\\~\\$
$\implies a(\dfrac{1+\sqrt{3}i}{2}) = b $
$\\~\\$

$v_2 = \begin{pmatrix} 1+\sqrt{3}i \\ 2 \end{pmatrix}$
$\\~\\$
$X(t) = \alpha e^{\lambda_1 t}  \begin{pmatrix} \sqrt{3}i - 1 \\ 2 \end{pmatrix} + \beta e^{\lambda_2 t}  \begin{pmatrix} \sqrt{3}i + 1 \\ 2 \end{pmatrix}$
$\\~\\$

What kind? 
$\\~\\$


$\\~\\$

The system of differential equations is given by: 

$\begin{pmatrix} \dot x \\ \dot y  \end{pmatrix} = \begin{pmatrix} 0 & 1 \\ -x & -y \end{pmatrix} = A \begin{pmatrix} x \\ y \end{pmatrix}$, 

where 

$A = \begin{pmatrix} 0 & 1 \\ -1 & -1 \end{pmatrix}$.

To find the eigenvalues of $A$, we solve the characteristic equation: 

$(-\lambda)(-\lambda -1)+1 = 0$.

This simplifies to $\lambda^2 + \lambda +1 = 0$, whose roots are $\lambda_1 = \dfrac{-1+\sqrt{3}i}{2}$ and $\lambda_2 = \dfrac{-1-\sqrt{3}i}{2}$.

To find the eigenvector corresponding to $\lambda_1$, we solve the equation: 

$\begin{pmatrix} \dfrac{-1-\sqrt{3}i}{2} & 1 \\ -1 & \dfrac{-1-\sqrt{3}i}{2}\end{pmatrix}\begin{pmatrix} a\\ b\end{pmatrix} = 0$.

This gives us $-a(\dfrac{1-\sqrt{3}i}{2})-ab = 0$, which simplifies to $a = -b\dfrac{(1+\sqrt{3}i)}{2}$. Solving for $b$, we obtain $b = \dfrac{-a(1-\sqrt{3}i)}{(1+\sqrt{3}i)(1-\sqrt{3}i)} = \dfrac{-a(1-\sqrt{3}i)}{2}$.

Therefore, an eigenvector for $\lambda_1$ is $v_1 = \begin{pmatrix} \sqrt{3}i - 1 \\ 2 \end{pmatrix}$.

Similarly, we can find an eigenvector for $\lambda_2$ by solving the equation: 

$\begin{pmatrix} \dfrac{1+\sqrt{3}i}{2} & 1 \\ -1 &  \dfrac{-1+\sqrt{3}i}{2}\end{pmatrix}\begin{pmatrix} a\\ b\end{pmatrix} = \begin{pmatrix} 0 \\ 0 \end{pmatrix}$.

This leads to the equations $a(\dfrac{1+\sqrt{3}i}{2}) = b$ and $-a = b (\dfrac{\sqrt{3}i - 1}{2})$, from which we can deduce that $a(\dfrac{1+\sqrt{3}i}{2}) = b$.

Thus, an eigenvector for $\lambda_2$ is $v_2 = \begin{pmatrix} 1+\sqrt{3}i \\ 2 \end{pmatrix}$.

Finally, the general solution to the system of differential equations is given by:

$X(t) = \alpha e^{\lambda_1 t}  \begin{pmatrix} \sqrt{3}i - 1 \\ 2 \end{pmatrix} + \beta e^{\lambda_2 t}  \begin{pmatrix} \sqrt{3}i + 1 \\ 2 \end{pmatrix}$,

where $\alpha$ and $\beta$ are constants. 
$\\~\\$
