## Theorem: For the linear differential equation \( \dot{x}=y \) and \( \dot{y}=-x-y). Prove that the origin is circulation.


## Proof: **(d)** $\dot{x} = y$ & $\dot{y} = -x - y$

$\implies \frac{d}{dt} \begin{bmatrix} x \\ y \end{bmatrix} = \begin{bmatrix} 0 & 1 \\ -1 & -1 \end{bmatrix} \begin{bmatrix} x \\ y \end{bmatrix}$

or 

$\dot{v} = A v$ where $A = \begin{bmatrix} 0 & 1 \\ -1 & -1 \end{bmatrix}$

characteristic equation of $A$ is 

$+ \lambda (\lambda + 1) + 1 = 0$

$\lambda^2 + \lambda + 1 = 0$

$\therefore \lambda_1 = \frac{-1 + i \sqrt{3}}{2} = e^{\frac{i 2 \pi}{3}}$

& $\lambda_2 = \frac{-1 - i \sqrt{3}}{2} = e^{\frac{i 4 \pi}{3}}$

To find the eigen vectors

$A v_1 = e^{\frac{i 2 \pi}{3}} v_1$

$e^{\frac{i 2 \pi}{3}} \begin{bmatrix} x \\ y \end{bmatrix} = \begin{bmatrix} 0 & 1 \\ -1 & -1 \end{bmatrix} \begin{bmatrix} x \\ y \end{bmatrix}$

$\implies y = x e^{\frac{i 2 \pi}{3}}$ & $-x - y = e^{\frac{i 2 \pi}{3}} y$ 
