## Theorem: For the linear differential equation \( \dot{x}=y \) and \( \dot{y}=-x-y). Prove that the origin is circulation.


## Proof: (d) $AX = \lambda X$

$\begin{bmatrix}0 & 1 \\ -1 & -1\end{bmatrix} \begin{bmatrix}x \\ y\end{bmatrix} = \begin{bmatrix}\lambda x \\ \lambda x - y\end{bmatrix}$

$det(A-\lambda I) = 0$

$det\begin{bmatrix}-\lambda & 1 \\ -1 & -1-\lambda\end{bmatrix} = 0$

$(-\lambda)(-1 - \lambda) + 1 = 0$

$\lambda^2 + \lambda + 1 = 0$

$\lambda^2 + \lambda + \frac{1}{4} = -\frac{3}{4}$

$\lambda = \frac{-1 \pm \sqrt{1^2 - 4}}{2}$

$\lambda = \frac{-1 \pm \sqrt{-3}}{2} = \frac{-1\pm\sqrt{3}i}{2}$

$\lambda_1 = \frac{-1 + \sqrt{3}i}{2}$, $\lambda_2 = \frac{-1 - \sqrt{3}i}{2}$

for $\lambda_1$ $(A - \lambda I)\begin{bmatrix}x \\ y\end{bmatrix} = \begin{bmatrix}0 \\ 0\end{bmatrix}$

$\begin{bmatrix}\frac{1}{2} - \frac{\sqrt{3}i}{2} & 1 \\ -1 & -1 + \frac{1}{2} - \frac{\sqrt{3}i}{2}\end{bmatrix} \begin{bmatrix}x \\ y\end{bmatrix} = \begin{bmatrix}0 \\ 0\end{bmatrix}$

$\begin{bmatrix}\frac{1-\sqrt{3}i}{2} & 1 \\ -1 & \frac{-1-\sqrt{3}i}{2}\end{bmatrix} \begin{bmatrix}x \\ y\end{bmatrix} = \begin{bmatrix}0 \\ 0\end{bmatrix}$

$(\frac{-1 - \sqrt{3}i}{2})(x) + y = 0$

$y = (\frac{-1+\sqrt{3}i}{2})x$

take eigen vectors are of form: $v_1 = (1, \frac{-1+\sqrt{3}i}{2})$

$X_1(t) = \lambda e^{\lambda_1 t} v_1$

$X_1(t) = \lambda e^{(\frac{-1+\sqrt{3}i}{2})t}$ $\begin{bmatrix}1 \\ \frac{-1 + \sqrt{3}i}{2}\end{bmatrix}$

$X_1(t) = \lambda e^{- \frac{1}{2}t} \begin{bmatrix}e^{\frac{\sqrt{3}i}{2}t} \\ e^{i(\frac{-\sqrt{3}}{2} + \frac{3}{2})t}\end{bmatrix}$

$X_1(t) = \lambda e^{\frac{-1}{2}t} \begin{bmatrix}cos(\frac{\sqrt{3}}{2}t) + isin(\frac{\sqrt{3}}{2}t) \\ e^{\frac{-\sqrt{3}i}{2}t + \frac{3i}{2}t}\end{bmatrix} = ...$

we can already see that the origin would be a spiral sink. 

$X(t) = c_1 X_{Re} + c_2 X_{Im}$


Let's analyze the provided solution step-by-step:

**(d)**  The problem aims to find the solution to the system of differential equations represented in matrix form as $AX = \lambda X$.

The matrix $A$ is given as $\begin{bmatrix}0 & 1 \\ -1 & -1\end{bmatrix}$. The first step is to find the eigenvalues  ($\lambda$) of the matrix $A$.

To find the eigenvalues, we solve the characteristic equation: $det(A-\lambda I) = 0$, where $I$ is the identity matrix.

This leads to the quadratic equation $\lambda^2 + \lambda + 1 = 0$.  Solving this quadratic equation, we find the eigenvalues: $\lambda_1 = \frac{-1 + \sqrt{3}i}{2}$ and $\lambda_2 = \frac{-1 - \sqrt{3}i}{2}$.

Next, we proceed to find the eigenvector corresponding to  $\lambda_1$. We substitute $\lambda_1$ back into the equation $(A - \lambda I)\begin{bmatrix}x \\ y\end{bmatrix} = \begin{bmatrix}0 \\ 0\end{bmatrix}$ and solve for the vector $\begin{bmatrix}x \\ y\end{bmatrix}$.

This results in the equation $(\frac{-1 - \sqrt{3}i}{2})(x) + y = 0$, which simplifies to $y = (\frac{-1+\sqrt{3}i}{2})x$. 

Choosing $x=1$, we get the eigenvector $v_1 = (1, \frac{-1+\sqrt{3}i}{2})$.

Finally, the general solution for $X_1(t)$ is expressed as $X_1(t) = \lambda e^{\lambda_1 t} v_1$. This is further simplified by substituting the values of $\lambda_1$ and $v_1$ and using Euler's formula to express the complex exponential in terms of trigonometric functions.

The solution suggests that the origin would be a spiral sink based on the form of the solution obtained.

The general solution of the system is given as a linear combination of the real and imaginary parts of the solution: $X(t) = c_1 X_{Re} + c_2 X_{Im}$. 
