## Theorem: Prove that the series \( \sum\_{n=1}^{\infty}(-1)^{n} \frac{(n+1)^{32}}{n!} \) is convergent


## Proof: Problem (b): $\sum\limits_{n=1}^\infty (-1)^n \frac{(n+1)^{32}}{n!}$

We must check if this series converges absolutely or not. 

$a_n = (-1)^n \frac{(n+1)^{32}}{n!}$

Therefore, $|a_n| = \frac{(n+1)^{32}}{n!}$. 

Now, 
$$\lim\limits_{n \to \infty} \frac{a_{n+1}}{a_n} = \lim\limits_{n \to \infty} \frac{\frac{((n+1)+1)^{32}}{(n+1)!}}{\frac{(n+1)^{32}}{n!}} = \lim\limits_{n \to \infty} \frac{(n+2)^{32}}{(n+1)^{32}} \cdot \frac{n!}{(n+1)!} = \lim\limits_{n \to \infty} \frac{(n+2)^{32}}{(n+1)^{32}} \cdot \frac{1}{n+1}$$
$$= \lim\limits_{n \to \infty} (\frac{n+2}{n+1})^{32} \times \frac{1}{n+1}$$

Now, as $n \to \infty$:  $n > 0$ / $n \neq 0$. We can divide both numerator, denominator by $n^{32}$. 

$$\lim\limits_{n \to \infty} \frac{a_{n+1}}{a_n} =  \lim\limits_{n \to \infty}(1 + \frac{1}{n})^{32} \times \frac{1}{n+1}$$
$$ = \lim\limits_{n \to \infty} \frac{(1 + \frac{1}{n})^{32}}{(1 + \frac{1}{n})^{32}} \times \lim\limits_{n \to \infty} \frac{1}{n+1} = \lim\limits_{n \to \infty} \frac{(1+\frac{1}{n})^{32}}{(1+\frac{1}{n})^{32} \times 0} = 0$$

We write this as $\lim\limits_{n \to \infty} 1 + \frac{1}{n}$ exists $= 0$. 

... $a_n$ converges absolutely. 

$\sum\limits_{n=1}^\infty a_n$ converges. 

Hence proved.
