## Theorem: Prove that the series \( \sum\_{n=1}^{\infty}(-1)^{n} \frac{(n+1)^{32}}{n!} \) is convergent


## Proof: b) $\sum_{n=1}^{\infty} \frac{(-1)^n(n+1)^{32}}{n!} = \sum b_n$

$\rightarrow \sum |b_n| = \frac{(n+1)^{32}}{n!}$

We use the ratio test as follows: 

$$lim_{n \rightarrow \infty} \frac{b_{n+1}}{b_n} = lim_{n \rightarrow \infty} \frac{\frac{(n+2)^{32} \times n!}{(n+1)!(n+1)^{32}}}{\frac{1}{n+1}} = lim_{n \rightarrow \infty} (\frac{n+2}{n+1})^{32} \frac{1}{n+1} = lim_{n \rightarrow \infty} (\frac{1 + \frac{2}{n}}{1 + \frac{1}{n}})^{32} \frac{1}{n+1}$$. 

As $lim_{n \rightarrow \infty} \frac{1}{n} = 0$, 

By using limit laws, $lim_{n \rightarrow \infty} (\frac{1 + \frac{2}{n}}{1 + \frac{1}{n}})^{32} = 1$ 

Also, $lim_{n \rightarrow \infty} \frac{1}{n+1} = 0$

$\rightarrow lim_{n \rightarrow \infty} \frac{b_{n+1}}{b_n} = 1 \times 0 = 0$

Therefore by using ratio test, we get that $\sum |b_n|$ converges. 

And as absolute convergence $\rightarrow$ convergence

$\sum b_n$ is convergent. 
