## Theorem: Prove that the series \( \sum\_{n=1}^{\infty}(-1)^{n} \frac{(n+1)^{32}}{n!} \) is convergent


## Proof: Consider the sequence $\{b_n\}_{n \in \mathbb{P}}$ such that $b_n = \frac{(n+1)^{32}}{n!}$ for all $n \in \mathbb{P}$. Then, for $n \in \mathbb{P}$,
 $$
 \frac{b_{n+1}}{b_n}=\frac{(n+2)^{32}}{(n+1)!} \cdot \frac{n!}{(n+1)^{32}}=\frac{(n+2)^{32}}{(n+1)^{32}} \cdot \frac{n!}{n+1}=\left( 1+\frac{1}{n+1}\right)^{32} \cdot \frac{1}{n+1}.
 $$

Since $\lim_{n \to \infty} \frac{1}{n} = 0$, $\lim_{n \to \infty} \frac{1}{n+1} = 0$. Thus,
 $$
 \lim_{n \to \infty} \left(1+\frac{1}{n+1}\right) = 1 + 0 = 1,
 $$
 and
 $$
 \lim_{n \to \infty} \left(1+\frac{1}{n+1}\right)^{32} = \left(\lim_{n \to \infty} \left(1+\frac{1}{n+1}\right)\right)^{32}=1^{32} = 1
 $$
 (by the limit laws).

Thus, 
$$
 \lim_{k \to \infty} \frac{b_{n+1}}{b_n}=(1)(0)=0.
 $$

Since $0<1$, $\sum b_n$ converges. Now, from the ratio test, the sequence
 $$
 \left| \frac{(-1)^n (n+1)^{32}}{n!}\right| = b_n
 $$ 
 for all $n \in \mathbb{P}$. Thus, the series $\sum \frac{(-1)^n (n+1)^{32}}{n!}$ converges absolutely. Therefore, the series converges. (Absolute convergence implies conditional convergence). 
