## Theorem: Prove that the series \( \sum\_{n=1}^{\infty}(-1)^{n} \frac{(n+1)^{32}}{n!} \) is convergent


## Proof: (b) $\sum\limits_{n=1}^\infty \frac{(-1)^n (n!)^{32}}{n!}$

Apply ratio test i) $\lim\limits_{n \to \infty} \frac{(-1)^{n+1} ((n+1)!)^{32}}{(n+1)!} = 0$ - from an assignment question

logic:
...(is after $n\geq 32$  $\frac{((n+1)(n!))^{32}}{n:(n-1)...(n-32)!...1}$ 
...very

ii) $\lim\limits_{n \to \infty} \frac{a_{n+1}}{a_n} = \lim\limits_{n \to \infty} \frac{(-1)^{n+1} \frac{((n+1)!)^{32}}{(n+1)!}}{(-1)^n \frac{(n!)^{32}}{n!}} = \lim\limits_{n \to \infty} (-1) \frac{((n+1)!)^{32}}{(n+1)!} \frac{n!}{(n!)^{32}}$ (where $a_n$ is $n^{th}$ term of corresponding sequence)

We know $\lim\limits_{n \to \infty} \frac{n!}{n+1} = 1$
$\lim\limits_{n \to \infty} \frac{(n+1)!}{n!} = \lim\limits_{n \to \infty} \frac{(n+1)n!}{n!} = 1 \Rightarrow \lim\limits_{n \to \infty} \frac{(n!)^{32}}{((n+1)!)^{32}} = 1$
and $\lim\limits_{n \to \infty} \frac{(n!)^{32}}{(n+1)!} = 0$

...$\lim\limits_{n \to \infty} \frac{a_{n+1}}{a_n} = 0 < 1$ - from algebra of limit of sequences
... by ratio test, $\sum\limits_{n=1}^\infty \frac{(-1)^n (n!)^{32}}{n!}$ converges.


The solution attempts to determine the convergence of the infinite series  $\sum\limits_{n=1}^\infty \frac{(-1)^n (n!)^32}{n!}$ using the ratio test. 

First, it calculates the limit $\lim\limits_{n \to \infty} \frac{(-1)^{n+1} ((n+1)!)^{32}}{(n+1)!}$, stating it equals 0 and citing an assignment question. 

Then, it computes the limit of the ratio of consecutive terms:
$\lim\limits_{n \to \infty} \frac{a_{n+1}}{a_n}$, where $a_n =  \frac{(-1)^n (n!)^32}{n!}$. After simplification, it  obtains $\lim\limits_{n \to \infty} (-1) \frac{((n+1)!)^{32}}{(n+1)!} \frac{n!}{(n!)^{32}}$. 

The proof then uses the known result  $\lim\limits_{n \to \infty} \frac{n!}{n+1} = 1$  and derives that $\lim\limits_{n \to \infty} \frac{(n!)^{32}}{((n+1)!)^{32}} = 1$. It also states that $\lim\limits_{n \to \infty} \frac{(n!)^{32}}{(n+1)!} = 0$. 

Finally, the solution concludes that $\lim\limits_{n \to \infty} \frac{a_{n+1}}{a_n} = 0$, which is less than 1. Therefore, by the ratio test, the series $\sum\limits_{n=1}^\infty \frac{(-1)^n (n!)^{32}}{n!}$ converges. 
