## Theorem: Let \( f:[0,1] \rightarrow \mathbb{R} \) be a Riemann integrable function. Then, prove that the function \( F:[0,1] \rightarrow \mathbb{R} \) given by
\[
F(x)=\int\_{0}^{x} f(t) d t
\]
is not differentiable at each \( x \in(0,1) \).


## Proof: ## Extracted Text with LaTeX

**Counterexample:**
$F(x) = \begin{cases} 0 & 0 \le x \le \frac{1}{2} \\ 1 & \frac{1}{2} < x \le 1 \end{cases}$. $f$ is $RI$ on $[0,1]$ as it is bounded by 1.
... $F(x) = \int\limits_0^x f(t) dt = \begin{cases} \int\limits_0^x 0 dt = 0 & 0 \le x \le \frac{1}{2} \\ \int\limits_0^{\frac{1}{2}} 0 dt +  \int\limits_{\frac{1}{2}}^x 1 dt = (x - \frac{1}{2})  & \frac{1}{2} < x \le 1 \end{cases}$ From splitting of limits
... $\int\limits_{\frac{1}{2}}^1 f dt = (G(b) - G(a))$ From 2nd F.T.C
(As $G(x) = x$ is primitive of $G'(x) = f(x) \implies$) and f is RI on $[\frac{1}{2}, x]$ $(\frac{1}{2} \le x \le 1)$
... $\int\limits_{\frac{1}{2}}^1 1 dt = (x - (\frac{1}{2})) = x - \frac{1}{2}$
... $F(x) = \begin{cases} 0 & 0 \le x \le \frac{1}{2} \\ x - \frac{1}{2} & \frac{1}{2} < x \le 1 \end{cases}$

**Claim:** $F$ is not diff. at $\frac{1}{2}$.
To the contrary say $F$ was diff at $\frac{1}{2}$.
... we would get $\lim\limits_{h \to 0} \frac{F(\frac{1}{2} + h) - F(\frac{1}{2})}{h} = \lim\limits_{h \to 0^+} \frac{F(\frac{1}{2} + h) - F(\frac{1}{2})}{h}$
$F(\frac{1}{2}) = 0$
$F(\frac{1}{2} + h) = 0$ when $h < 0$ and in allowed value, i.e. $h > \frac{-1}{2}$
... $\lim\limits_{h \to 0^-} \frac{F(\frac{1}{2} + h) - F(\frac{1}{2})}{h} = \lim\limits_{h \to 0^-} \frac{0}{h} = 0$
**But** $F(\frac{1}{2} + h) = \frac{1}{2} + h - (\frac{1}{2}) = h$ when $h > 0$ and $h \le \frac{1}{2}$
... $\lim\limits_{h \to 0^+} \frac{F(\frac{1}{2} + h) - F(\frac{1}{2})}{h} = \lim\limits_{h \to 0^+} \frac{h - 0}{h} = \lim\limits_{h \to 0^+} 1 = 1$
as $0 \ne 1$ $\lim\limits_{h \to 0^-} \frac{F(\frac{1}{2} + h) - F(\frac{1}{2})}{h} \ne \lim\limits_{h \to 0^+} \frac{F(\frac{1}{2} + h) - F(\frac{1}{2})}{h}$
... $F$ is not diff at $\frac{1}{2}$.


## Cleaned Mathematical Proof

**Counterexample:**

Consider the function $F(x)$ defined as follows:
$$F(x) = \begin{cases} 
0 & 0 \le x \le \frac{1}{2} \\ 
1 & \frac{1}{2} < x \le 1 
\end{cases}$$
The function $f$ is Riemann Integrable (RI) on the interval $[0,1]$ as it is bounded by 1.

We can express $F(x)$ using the integral:
$$F(x) = \int\limits_0^x f(t) dt$$
By splitting the limits of integration, we get:
$$F(x) = \begin{cases} 
\int\limits_0^x 0 dt = 0 & 0 \le x \le \frac{1}{2} \\ 
\int\limits_0^{\frac{1}{2}} 0 dt +  \int\limits_{\frac{1}{2}}^x 1 dt = (x - \frac{1}{2})  & \frac{1}{2} < x \le 1 
\end{cases}$$

From the Second Fundamental Theorem of Calculus, we know:
$$\int\limits_{\frac{1}{2}}^1 f dt = (G(b) - G(a))$$
where $G(x) = x$ is the primitive of $G'(x) = f(x)$. 

Since $f$ is RI on  $[\frac{1}{2}, x]$ where $\frac{1}{2} \le x \le 1$, we have:
$$\int\limits_{\frac{1}{2}}^1 1 dt = (x - (\frac{1}{2})) = x - \frac{1}{2}$$

Therefore, we can rewrite $F(x)$ as:
$$F(x) = \begin{cases} 
0 & 0 \le x \le \frac{1}{2} \\ 
x - \frac{1}{2} & \frac{1}{2} < x \le 1 
\end{cases}$$

**Claim:**

The function $F$ is not differentiable at $x = \frac{1}{2}$.

**Proof by contradiction:**

Assume, to the contrary, that $F$ is differentiable at $x = \frac{1}{2}$. 

This would imply that the following limit exists:
$$\lim\limits_{h \to 0} \frac{F(\frac{1}{2} + h) - F(\frac{1}{2})}{h}$$
which is equivalent to:
$$\lim\limits_{h \to 0^+} \frac{F(\frac{1}{2} + h) - F(\frac{1}{2})}{h}$$

We know that $F(\frac{1}{2}) = 0$. 

When $h < 0$ and within the allowed values, specifically $h > \frac{-1}{2}$, we have: 
$$F(\frac{1}{2} + h) = 0$$

Therefore, the left-hand limit becomes:
$$\lim\limits_{h \to 0^-} \frac{F(\frac{1}{2} + h) - F(\frac{1}{2})}{h} = \lim\limits_{h \to 0^-} \frac{0}{h} = 0$$

**However**, when $h > 0$ and $h \le \frac{1}{2}$, we have:
$$F(\frac{1}{2} + h) = \frac{1}{2} + h - (\frac{1}{2}) = h$$

This leads to the right-hand limit:
$$\lim\limits_{h \to 0^+} \frac{F(\frac{1}{2} + h) - F(\frac{1}{2})}{h} = \lim\limits_{h \to 0^+} \frac{h - 0}{h} = \lim\limits_{h \to 0^+} 1 = 1$$

Since $0 \ne 1$, we have:
$$\lim\limits_{h \to 0^-} \frac{F(\frac{1}{2} + h) - F(\frac{1}{2})}{h} \ne \lim\limits_{h \to 0^+} \frac{F(\frac{1}{2} + h) - F(\frac{1}{2})}{h}$$

This contradicts our initial assumption that $F$ is differentiable at $x = \frac{1}{2}$. Therefore, $F$ is not differentiable at $x = \frac{1}{2}$. 
