## Theorem: For the linear differential equation \( \dot{x}=-y \) and \( \dot{y}=x). Prove that the origin is circulation.


## Proof: (c) $\dot{x} = -y$
$\dot{y} = x$

$\begin{bmatrix} \dot{x} \\ \dot{y} \end{bmatrix} = \begin{bmatrix} 0 & -1 \\ 1 & 0 \end{bmatrix} \begin{bmatrix} x \\ y \end{bmatrix}$

$\dot{X} = AX$

$|A-\lambda I| = 0$

$\implies \begin{vmatrix} -\lambda & -1 \\ 1 & -\lambda \end{vmatrix} = 0$

$\implies \lambda^2 + 1 = 0$

$\implies \lambda^2 = -1 \implies \lambda = \pm i \qquad$ COMPLEX EIGENVALUES

for $\lambda = i$
$\begin{bmatrix} -i & -1 \\ 1 & -i \end{bmatrix} \begin{bmatrix} x \\ y \end{bmatrix} = 0$
$\implies \begin{aligned} -xi - y &= 0 \\ x-iy &=0 \end{aligned} \implies x =iy \qquad \begin{pmatrix} i \\ 1 \end{pmatrix}$

for $\lambda = -i$
$\begin{bmatrix} i & -1 \\ 1 & i \end{bmatrix} \begin{bmatrix} x \\ y \end{bmatrix} = 0$
$\implies xi-y = 0 \implies x = \begin{pmatrix} 1 \\ i \end{pmatrix}$

General Soln:
$X(t) = \vec{V_1}e^{\lambda t} + \vec{V_2}e^{\lambda t}$

$=  \alpha \begin{pmatrix} i \\ 1 \end{pmatrix} (\cos t + i \sin t) + \beta \begin{pmatrix} 1 \\ i \end{pmatrix} (\cos t -i \sin t)$

$= \alpha \begin{pmatrix} i\cos t - \sin t \\ \cos t + i \sin t \end{pmatrix} + \beta \begin{pmatrix} \cos t - i \sin t \\ i \cos t + \sin t \end{pmatrix}$

$= \begin{pmatrix} \beta \cos t - \alpha \sin t + i (\alpha \cos t - \beta \sin t)\\ \alpha \cos t + \beta \sin t + i(\alpha \sin t + \beta \cos t) \end{pmatrix}$

$x^2 + y^2 = a$

$x$, $t$ is a function of $\alpha$ and $\beta$ only and not $t$. Also, $y$ and $x$ are periodic functions. These equations and conditions satisfy the trajectory of a circle. The distance from the origin remains the same with time $t$, only the phase changes. 

Anti-clockwise for $\alpha < 0$
Clockwise for $\beta < 0$

origin is a 
CIRCULATION

Let's break down the solution step by step:

**(c)** We are given a system of differential equations:

* $\dot{x} = -y$ 
* $\dot{y} = x$

This system can be represented in matrix form as:

$\begin{bmatrix} \dot{x} \\ \dot{y} \end{bmatrix} = \begin{bmatrix} 0 & -1 \\ 1 & 0 \end{bmatrix} \begin{bmatrix} x \\ y \end{bmatrix}$

which can be written concisely as:

$\dot{X} = AX$

where $\dot{X} = \begin{bmatrix} \dot{x} \\ \dot{y} \end{bmatrix}$ and  $A = \begin{bmatrix} 0 & -1 \\ 1 & 0 \end{bmatrix}$.

To find the eigenvalues of matrix A, we solve the characteristic equation:

$|A-\lambda I| = 0$

This expands to:

$\begin{vmatrix} -\lambda & -1 \\ 1 & -\lambda \end{vmatrix} = 0$

Calculating the determinant, we get:

$\implies \lambda^2 + 1 = 0$

Solving for $\lambda$, we find:

$\implies \lambda^2 = -1 \implies \lambda = \pm i $

Therefore, the eigenvalues are complex conjugates: $\lambda = i$ and $\lambda = -i$.

**For $\lambda = i$:**

We substitute $\lambda = i$ back into the equation $(A-\lambda I)\begin{bmatrix} x \\ y \end{bmatrix} = 0$ and get:

$\begin{bmatrix} -i & -1 \\ 1 & -i \end{bmatrix} \begin{bmatrix} x \\ y \end{bmatrix} = 0$

This matrix equation corresponds to the system of equations:

$\begin{aligned} -xi - y &= 0 \\ x-iy &=0 \end{aligned}$

Solving this system, we find a relationship between x and y:  $x =iy$.  An eigenvector corresponding to this eigenvalue is $\begin{pmatrix} i \\ 1 \end{pmatrix}$. 

**For $\lambda = -i$:**

Similarly, for  λ=−i, we substitute it into $(A−λI)\begin{bmatrix} x \\ y \end{bmatrix}=0$ to get:

$\begin{bmatrix} i & -1 \\ 1 & i \end{bmatrix} \begin{bmatrix} x \\ y \end{bmatrix} = 0$

This gives us the equation: $xi-y=0$.  An eigenvector corresponding to this eigenvalue is $\begin{pmatrix} 1 \\ i \end{pmatrix}$.

**General Solution:**

The general solution of the system of differential equations is given by:

$X(t) = \vec{V_1}e^{\lambda_1 t} + \vec{V_2}e^{\lambda_2 t}$

Substituting the eigenvalues and eigenvectors we found, the general solution becomes:

$X(t) =  \alpha \begin{pmatrix} i \\ 1 \end{pmatrix} (\cos t + i \sin t) + \beta \begin{pmatrix} 1 \\ i \end{pmatrix} (\cos t -i \sin t)$

where α and β are arbitrary constants.

Expanding and rearranging the terms, we get:

$X(t) = \alpha \begin{pmatrix} i\cos t - \sin t \\ \cos t + i \sin t \end{pmatrix} + \beta \begin{pmatrix} \cos t - i \sin t \\ i \cos t + \sin t \end{pmatrix}$

$X(t) = \begin{pmatrix} \beta \cos t - \alpha \sin t + i (\alpha \cos t - \beta \sin t)\\ \alpha \cos t + \beta \sin t + i(\alpha \sin t + \beta \cos t) \end{pmatrix}$

The solution implies:

$x^2 + y^2 = a$, where $a$ is a constant.

We observe that:

* $x$ is a function of $\alpha$ and $\beta$ only, and not explicitly dependent on  $t$.
* $y$ is also a function of $\alpha$ and $\beta$ only.
* Both $x$ and $y$ are periodic functions.

These observations, along with the equation $x^2+y^2=a$, suggest that the trajectory of the solution in the phase plane is a circle centered at the origin. 

The distance from the origin remains constant over time, only the phase of the solution changes.

The direction of motion along the circular trajectory depends on the signs of $\alpha$ and $\beta$:

* The motion is anti-clockwise for $\alpha < 0$.
* The motion is clockwise for $\beta < 0$.

The origin is a point of circulation for the system.
