## Theorem: For the linear differential equation \( \dot{x}=-y \) and \( \dot{y}=x). Prove that the origin is circulation.


## Proof: We have $j = n$.  Then $\frac{dy}{dn} = n$ so that $dy = ndn$.  Therefore, $\int dy = \int ndn$, which implies that $y = \frac{n^2}{2}$.

We also have $i = -y$.  Thus $\frac{dn}{dy} = -y$ so that $dn = -y dy$.  Hence, $\int dn = \int -y dy$.  This gives us $n = \frac{-y^2}{2}$.  Then $2n = -y^2$.  Hence $y^2 + 2n = 0$.

We have that $y = \frac{n^2}{2}$.  Then $2y = n^2$, so $n^2 - 2y = 0$.

We can substitute to get $y^2 + 2n = n^2 - 2y$.  Rearranging, we get $n^2 - y^2 - 2n - 2y = 0$.  Factoring, we obtain $n^2 - 2n - (y^2 + 2y) = 0$.  Thus $n^2 - 2n - (y^2 + 2y) = 0 = f$.

Therefore $\nabla f = 2n - 2 - (2y + 2) = 2n - 2y - 4$.  At the origin, $\nabla f = -4$.  Therefore, at the origin, it is a source.