## Theorem: For the linear differential equation \( \dot{x}=-y \) and \( \dot{y}=x). Prove that the origin is circulation.


## Proof: **Extracted Text in LaTeX:**

\begin{align*}
\frac{d}{dt} \begin{bmatrix} x \\ y \end{bmatrix} &= \begin{bmatrix} 0 & -1 \\ 1 & 0 \end{bmatrix} \begin{bmatrix} x \\ y \end{bmatrix} \\
&= A \mathbf{v} \quad \text{where } A = \begin{bmatrix} 0 & -1 \\ 1 & 0 \end{bmatrix} \\
\lambda^2 &= -1 \\
\lambda_1 &= i, \ \lambda_2 = -i \\
A\mathbf{v}_1 &= \begin{bmatrix} 0 & -1 \\ 1 & 0 \end{bmatrix} \begin{bmatrix} 1 \\ i \end{bmatrix} = i \begin{bmatrix} 1 \\ i \end{bmatrix} \\
&\implies -y = ix \text{ and } x = iy \\
&\implies \mathbf{v}_1 = \begin{bmatrix} 1 \\ i \end{bmatrix} \\
A\mathbf{v}_2 &= \begin{bmatrix} 0 & -1 \\ 1 & 0 \end{bmatrix} \begin{bmatrix} 1 \\ -i \end{bmatrix} = \begin{bmatrix} i \\ 1 \end{bmatrix} \\
&\implies -y = -ix \text{ and } x = -iy \\
&\implies \mathbf{v}_2 = \begin{bmatrix} 1 \\ -i \end{bmatrix} \\
\frac{d}{dt} \begin{bmatrix} x \\ y \end{bmatrix} &= \begin{bmatrix} 0 & -1 \\ 1 & 0 \end{bmatrix} \begin{bmatrix} x \\ y \end{bmatrix} = \begin{bmatrix} 0 & -1 \\ 1 & 0 \end{bmatrix} \begin{bmatrix} c_1(1) + c_2(1) \\ c_1(i) + c_2(-i) \end{bmatrix} \\
\frac{dx}{dt} &= -i x \implies x = c_1 e^{it} \\
\frac{dy}{dt} &= -iy \implies y = c_2 e^{-it} 
\end{align*}

**Clean Mathematical Proof:**

We are given the following system of differential equations:
$$\frac{dx}{dt} = -y$$
$$\frac{dy}{dt} = x$$

We can rewrite this system in matrix form:

$$\frac{d}{dt} \begin{bmatrix} x \\ y \end{bmatrix} = \begin{bmatrix} 0 & -1 \\ 1 & 0 \end{bmatrix} \begin{bmatrix} x \\ y \end{bmatrix}$$

Let's denote the matrix by $A = \begin{bmatrix} 0 & -1 \\ 1 & 0 \end{bmatrix}$.  To find the general solution, we will find the eigenvalues and eigenvectors of $A$.

The characteristic equation of $A$ is:

$$\text{det}(A - \lambda I) = \begin{vmatrix} -\lambda & -1 \\ 1 & -\lambda \end{vmatrix} = \lambda^2 + 1 = 0$$

Solving for $\lambda$, we get two complex eigenvalues:

$$\lambda_1 = i, \quad \lambda_2 = -i$$

Now, let's find the eigenvector corresponding to $\lambda_1 = i$. We need to solve the following system:

$$(A - iI)\mathbf{v}_1 = \mathbf{0}$$

This simplifies to:

$$\begin{bmatrix} -i & -1 \\ 1 & -i \end{bmatrix} \begin{bmatrix} v_{11} \\ v_{12} \end{bmatrix} = \begin{bmatrix} 0 \\ 0 \end{bmatrix}$$

Solving this system, we find that an eigenvector corresponding to $\lambda_1 = i$ is:

$$\mathbf{v}_1 = \begin{bmatrix} 1 \\ i \end{bmatrix}$$

Similarly, we can find the eigenvector corresponding to $\lambda_2 = -i$:

$$\mathbf{v}_2 = \begin{bmatrix} 1 \\ -i \end{bmatrix}$$

Since we have two linearly independent eigenvectors, the general solution of the system is given by:

$$\begin{bmatrix} x(t) \\ y(t) \end{bmatrix} = c_1 e^{it} \mathbf{v}_1 + c_2 e^{-it} \mathbf{v}_2 =  c_1 e^{it} \begin{bmatrix} 1 \\ i \end{bmatrix} + c_2 e^{-it} \begin{bmatrix} 1 \\ -i \end{bmatrix}$$

where $c_1$ and $c_2$ are arbitrary constants.

Expanding this expression, we get:

$$x(t) = c_1 e^{it} + c_2 e^{-it}$$
$$y(t) = c_1 i e^{it} - c_2 i e^{-it}$$

These equations describe a circular trajectory in the $xy$-plane, as the real and imaginary parts of $e^{it}$ and $e^{-it}$ represent cosine and sine functions, respectively. Therefore, the trajectory of the system is a circle. 
