## Theorem: For the linear differential equation \( \dot{x}=-y \) and \( \dot{y}=x). Prove that the origin is circulation.


## Proof: $AX = X'$

$\begin{bmatrix} 0 & -1 \\ 1 & 0 \end{bmatrix} \begin{bmatrix} x \\ y \end{bmatrix} = \begin{bmatrix} -y \\ x \end{bmatrix}$

$ det (A - \lambda I) = 0$

$ det \left( \begin{bmatrix} 0 & -1 \\ 1 & 0 \end{bmatrix} + \begin{bmatrix} -\lambda & 0 \\ 0 & -\lambda \end{bmatrix} \right) = 0$

$ det \begin{bmatrix} -\lambda & -1 \\ 1 & -\lambda \end{bmatrix} = 0$

$\lambda^2 + 1 = 0$

$\lambda^2 = -1$

$\lambda = \pm i$

$ for \ \lambda_1 = i$ & $\lambda_2 = -i$

$ \begin{bmatrix} -i & -1 \\ 1 & -i \end{bmatrix} \begin{bmatrix} x \\ y \end{bmatrix} = \begin{bmatrix} 0 \\ 0 \end{bmatrix}$

$ -ix - y = 0$

$ +x -iy = 0$  $same$

$ x = iy$

Thus we take eigen vector as $\begin{bmatrix} 1 \\ -i \end{bmatrix}$ when $\lambda_1 = i$ but we can't have it

$ X(t) = e^t \begin{bmatrix} 1 \\ -i \end{bmatrix}$ 

but we can't have complex solutions to real equations

$e^{i \theta} = (i sin \theta + cos \theta)$

$X(t) = \begin{bmatrix} e^{it} \\ -i e^{it} \end{bmatrix}$

$X(t) = \begin{bmatrix} i sin \theta + cos \theta \\ -i^2 sin \theta - i cos \theta \end{bmatrix}$

$X(t) = \begin{bmatrix} i sin \theta + cos \theta \\ sin \theta - i cos \theta \end{bmatrix}$

where $\theta = t$ 

$\implies$ 

$X(t) = \begin{bmatrix} cos \theta \\ sin \theta \end{bmatrix} + i \begin{bmatrix} sin \theta \\ -cos \theta \end{bmatrix}$

$\theta = t$ 

$X_{Re} = \begin{bmatrix} cos \theta \\ sin \theta \end{bmatrix}$ $X_{im} = \begin{bmatrix} sin \theta \\ -cos \theta \end{bmatrix}$

Thus this an eq of circulation origin 

$X(t) = c_1 X_{Re} + c_2 X_{im}$

---

We are given the system of differential equations $AX=X'$ where $A = \begin{bmatrix} 0 & -1 \\ 1 & 0 \end{bmatrix}$.  To solve this, we will find the eigenvalues and eigenvectors of $A$. 

The eigenvalues are the solutions to the characteristic equation $ det (A - \lambda I) = 0$.  Expanding this determinant, we get the equation $\lambda^2 + 1 = 0$, which gives us eigenvalues of $\lambda = \pm i$.

Let's start with the eigenvalue  $\lambda_1 = i$.  Plugging this into the equation $(A-\lambda I)X = 0$ gives us  $ \begin{bmatrix} -i & -1 \\ 1 & -i \end{bmatrix} \begin{bmatrix} x \\ y \end{bmatrix} = \begin{bmatrix} 0 \\ 0 \end{bmatrix}$. This system simplifies to the equation $x=iy$. Thus, the eigenvector corresponding to $\lambda_1 = i$ is $\begin{bmatrix} 1 \\ -i \end{bmatrix}$. 

A solution to the system of differential equations could then be given by $X(t) = e^t \begin{bmatrix} 1 \\ -i \end{bmatrix}$. However, this solution involves complex numbers and we are seeking real solutions. 

Using Euler's formula, we can rewrite $e^{it}$ as $e^{i \theta} = (i sin \theta + cos \theta)$.  Substituting this into our expression for $X(t)$ and simplifying gives us $X(t) = \begin{bmatrix} i sin \theta + cos \theta \\ sin \theta - i cos \theta \end{bmatrix}$ where $\theta = t$.

We can rewrite this solution as $X(t) = \begin{bmatrix} cos \theta \\ sin \theta \end{bmatrix} + i \begin{bmatrix} sin \theta \\ -cos \theta \end{bmatrix}$ where $\theta = t$.  We can then express this as $X(t) = c_1 X_{Re} + c_2 X_{im}$, where  $X_{Re} = \begin{bmatrix} cos \theta \\ sin \theta \end{bmatrix}$ and $X_{im} = \begin{bmatrix} sin \theta \\ -cos \theta \end{bmatrix}$. This solution describes a circulation about the origin. 
