## Theorem: Let \( A, B \subset \mathbb{R} \) be nonempty sets that are bounded above. Then prove that \( A \cup B \) is nonempty and bounded above, and
\[
\sup (A \cup B)=\max \{\sup A, \sup B\}
\]


## Proof: I attempt to prove this statement by means of contradiction. Let $\sup A = c$ and $\sup B = d$ where $c, d \in \mathbb{R}$. Now also let $\sup(A \cup B) = e$ such that $e \neq \max\{c, d\}$. 

**Case I**  $e \in A$. 

This implies $e \gamma c$ and hence $\sup A = e$, which contradicts our initial assumption of $\sup A = c$ provided $e \neq c$.

**Case II**  $e \in B$. 

This implies $e \gamma d$ and hence $\sup B = e$, which contradicts our initial assumption of $\sup B = d$ provided $e \neq d$. 

may be neither in $A$, nor in $B$.

From both cases, it is clear $\nexists \ e$ satisfying the set of conditions $\sup (A \cup B) = d \ni e; \ e \neq \{\sup A, \sup B\} \ \forall \ e \in \mathbb{R}$.

which in turn implies 

$\sup (A \cup B) = \max \{\sup A, \sup B\}$ (Hence, proven).

## Cleaned-up Proof:

We attempt to prove the statement by means of contradiction. Let $\sup A = c$ and $\sup B = d$ where $c, d \in \mathbb{R}$. Now, let $\sup(A \cup B) = e$ such that $e \neq \max\{c, d\}$. 

**Case I:**  Assume $e \in A$. 

This implies $e \leq c$ and hence $\sup A = e$, which contradicts our initial assumption that $\sup A = c$ since we assumed $e \neq \max\{c,d\}$.

**Case II:**  Assume $e \in B$. 

This implies $e \leq d$ and hence $\sup B = e$, which contradicts our initial assumption that $\sup B = d$ since we assumed $e \neq \max\{c,d\}$. 

From both cases, we see that there does not exist an $e$ satisfying the set of conditions $\sup (A \cup B) = e$ where $e \neq \sup A$ and $e \neq \sup B$ for all $e \in \mathbb{R}$.

This, in turn, implies that 
$\sup (A \cup B) = \max \{\sup A, \sup B\}$.  Hence, the statement is proven. 
