## Theorem: Let \( A, B \subset \mathbb{R} \) be nonempty sets that are bounded above. Then prove that \( A \cup B \) is nonempty and bounded above, and
\[
\sup (A \cup B)=\max \{\sup A, \sup B\}
\]


## Proof: WLOG let $\sup A \ge \sup B$ $\qquad \circled{1}$ 
(If not, then replace $A$ by $B$ and $B$ by $A$ in following proof.)

$\because A \subseteq A \cup B$ 
$\therefore$ Since $A$ is non empty, $A \cup B$ is non empty.
By def$^{n}$, $\forall x \in A \qquad x\le \sup (A)$ as $\sup(A)$ is UB of $A$
and $\qquad \forall y \in B \qquad y\le \sup(B) \le \sup(A)$ and $\sup (B)$ is UB of $B$
$\qquad \qquad \qquad \qquad  \qquad \qquad  \qquad \qquad \qquad$  $\because \sup B \le \sup A\qquad\circled{1}$

$\therefore \forall z \in A \cup B,\quad z \le \sup (A)$
$\therefore \sup (A)$ is UB of $A\cup B \qquad \circled{2}$
$\because A \cup B$ is non empty and bold above it admits a supremum 
$\therefore \sup (A)$ is supremum of $A$, by definition, 
$\forall \varepsilon > 0 \quad \exists \  x \in A \subseteq A\cup B$ s.t. $\qquad x > \sup (A) - \varepsilon$
$\forall \varepsilon > 0 \quad \exists \ x \in A \cup B$ s.t $\qquad x> \sup (A) - \varepsilon \qquad \circled{3}$
From $\circled{2}$ and $\circled{3}$ $\qquad  \sup (A \cup B) = \sup A \qquad \circled{4}$ (If $\sup A \ge \sup B$ 
(repeat, exchange $A$ and $B$ if $\sup A < \sup B$ in above proof)

**EXTRA SPACE FOR PROBLEM 1 (a)**

$\therefore$ if $\sup B \ge \sup (A)$ we get (from exchange)

$\sup (A \cup B) = \sup (B) \qquad \circled{5}$

$\therefore$ From $\circled{4}$ and $\circled{5}$ 

$\sup (A \cup B) = \max \{\sup (A), \sup (B) \}$



**Cleaned-up Proof:**

Without loss of generality, let $\sup A \ge \sup B$. (If not, then exchange $A$ by $B$ and $B$ by $A$ in the following proof).

Because $A \subseteq A \cup B$, and $A$ is non-empty,  $A \cup B$ is non-empty. 
By definition, $\forall x \in A$, $x \le \sup(A)$, as $\sup(A)$ is an upper bound of $A$. Similarly,  $\forall y \in B$, $ y \le \sup(B) \le \sup(A)$, as $\sup (B)$ is an upper bound of $B$ and $\sup B \le \sup A$.

Therefore, $\forall z \in A \cup B$, $z \le \sup (A)$. 
Thus, $\sup (A)$ is an upper bound of $A\cup B$. 

Because $A \cup B$ is non-empty and bounded above, it admits a supremum. 
By definition of the supremum, $\forall \varepsilon > 0$, $\exists \  x \in A \subseteq A\cup B$ such that $x > \sup (A) - \varepsilon$. 
Equivalently, $\forall \varepsilon > 0$, $\exists \ x \in A \cup B$ such that $x> \sup (A) - \varepsilon$. 

From the above statements, we conclude that  $\sup (A \cup B) = \sup A$. (If $\sup A \ge \sup B$. The proof for the case where $\sup A < \sup B$ is obtained by exchanging $A$ and $B$ in the above argument).

Now, if $\sup B \ge \sup (A)$, we get by exchanging $A$ and $B$ that  $\sup (A \cup B) = \sup (B)$.

Therefore, from the two cases, we have  $\sup (A \cup B) = \max \{\sup (A), \sup (B) \}$. 
