## Theorem: Let \( f(x, y)=x^{3}-3 x+y^{2} \) for \( x, y \in \mathbb{R} \). Prove that at the points (1,0) and (-1,0) the gradient of \( f \) is zero.


## Proof: Problem 2:
$f(x,y) = x^3 - 3x + y^2$

(a) $\nabla f = \mathbf{0}$

$\implies (\frac{\partial f}{\partial x}\mathbf{i} + \frac{\partial f}{\partial y}\mathbf{j}) = \mathbf{0}\mathbf{i} + \mathbf{0}\mathbf{j}$

So $\frac{\partial f}{\partial x} = 3x^2 - 3 = 0$
$\implies x^2 = 1 \implies x = \pm 1$

$\frac{\partial f}{\partial y} = 2y = 0 \implies y=0$.

Hence the points at which $\text{grad}(f)$ is zero are $(1,0)$ & $(-1,0)$.

$\nabla f = (3x^2 - 3)\mathbf{i} + 2y\mathbf{j}$ 
