## Theorem: Let \( f(x, y)=x^{3}-3 x+y^{2} \) for \( x, y \in \mathbb{R} \). Prove that at the points (1,0) and (-1,0) the gradient of \( f \) is zero.


## Proof: Let  $f(x,y) = x^3 - 3x + y^2$.  The gradient of $f$ is 
$$\nabla f(x,y) = \left( \frac{\partial f}{\partial x} \hat{i} +  \frac{\partial f}{\partial y} \hat{j} \right) = (3x^2 - 3) \hat{i} + 2y \hat{j}.$$  Setting the gradient equal to zero gives 
$$(3x^2 - 3) \hat{i} + 2y \hat{j} = 0.$$  We can set each component equal to zero individually to get the system of equations 
\begin{align*}
3x^2 - 3 &= 0 \\
2y &= 0. 
\end{align*} Solving, we find that $x = \pm 1$ and $y=0$.  Therefore, the points $(x,y)$ are $(1,0)$ and $(-1,0)$. 
