## Theorem: Let \( f(x, y)=x^{3}-3 x+y^{2} \) for \( x, y \in \mathbb{R} \). Prove that at the points (1,0) and (-1,0) the gradient of \( f \) is zero.


## Proof: Let $f(x, y) = x^3 - 3x + y^2$ for all $x, y \in \mathbb{R}$. 

**(a)** Then $ \nabla f(x, y) = \frac{\partial f(x, y)}{\partial x} \hat{i} + \frac{\partial f(x, y)}{\partial y} \hat{j}$. 

$\implies \nabla f(x, y) = (3x^2 - 3) \hat{i} + (2y) \hat{j}$. 

Thus, $\nabla f(x, y) = 0$. 

$\implies 3x^2 - 3 = 0$ and $2y = 0$.

$\implies x = 1$ and $y = 0$ or $x=-1$ and $y=0$.

Therefore, $(x, y) = \{(1, 0), (-1, 0)\}$. 
