## Theorem: For the linear differential equation \( \dot{x}=x \) and \( \dot{y}=y). Prove that the origin is source.


## Proof: (b) $\dot{x} = x$
$\dot{y} = y$.
$\frac{dx}{dy} = x$
$\frac{dy}{dx} = y$.
$\frac{1}{x} dx = dy$
$\frac{1}{y} dy = dx$.
$log\,x = y$.
$log\,y = x$.
$log\,x - y = 0$
$log\,y - x = 0$.

$log\,x - y = log\,y - x$.
$log\,x - log\,y + x - y = 0$.
$log(\frac{x}{y}) + x - y = 0$.
$log(\frac{x}{y}) = y - x$.

$\frac{x}{y} = e^{y-x}$.

$\frac{x}{y} = \frac{e^y}{e^x}$.
$x e^x = y e^y$.
$x e^x - y e^y = 0. = f$.
$\nabla f =  xe^x + e^x - (ye^y + e^y)$
$= e^x(x+1) - e^y(y+1)$
At origin
$\nabla f = 0$
$\therefore$ The origin will be a saddle.

---

**(b)** We have $\dot{x} = x$ and $\dot{y} = y$. Then $\frac{dx}{dy} = x$ and $\frac{dy}{dx} = y$. Rearranging, we get $\frac{1}{x} dx = dy$ and $\frac{1}{y} dy = dx$. Integrating, we have $log\,x = y$ and $log\,y = x$. This implies $log\,x - y = 0$ and $log\,y - x = 0$. 

Therefore, $log\,x - y = log\,y - x$. Combining terms, we get $log\,x - log\,y + x - y = 0$. Using log properties, we have $log(\frac{x}{y}) + x - y = 0$. That is, $log(\frac{x}{y}) = y - x$.

Exponentiating both sides, we get $\frac{x}{y} = e^{y-x}$. This can be rewritten as $\frac{x}{y} = \frac{e^y}{e^x}$, which gives us $x e^x = y e^y$. Rearranging, we have $x e^x - y e^y = 0$. Let this be denoted by $f$. Then, $\nabla f =  xe^x + e^x - (ye^y + e^y) = e^x(x+1) - e^y(y+1)$. At the origin, $\nabla f = 0$. Therefore, the origin will be a saddle. 
