## Theorem: For the linear differential equation \( \dot{x}=x \) and \( \dot{y}=y). Prove that the origin is source.


## Proof: $5(b)$

$AX = x'$

$\begin{bmatrix} 1 & 0 \\ 0 & 1 \end{bmatrix} \begin{bmatrix} x \\ y \end{bmatrix} = \begin{bmatrix} x \\ y \end{bmatrix}$

$det(A - dI) = 0$

$\implies det \begin{bmatrix} 1-d & 0 \\ 0 & 1-d \end{bmatrix} = 0$

$(1-d)(1-d) = 0$

$d = 1$

Thus $d_1 = d_2 = 1$

---

$(A - I)\begin{bmatrix} c_1 \\ c_2 \end{bmatrix} = \begin{bmatrix} 0 \\ 0 \end{bmatrix}$

$\begin{bmatrix} 0 & 0 \\ 0 & 0 \end{bmatrix} \begin{bmatrix} c_1 \\ c_2 \end{bmatrix} = \begin{bmatrix} 0 \\ 0 \end{bmatrix}$

Thus Above $v$ stops for $\forall v \in \mathbb{R}^2$ 

Let us take $v_1 = \begin{bmatrix} 1 \\ 1 \end{bmatrix}$ is base of solutions

$X(t) = \lambda e^t \begin{bmatrix} 1 \\ 1 \end{bmatrix}$ and is general solution 

----

For question 5(b), we have $AX = x'$ where  $A = \begin{bmatrix} 1 & 0 \\ 0 & 1 \end{bmatrix}$ and $X = \begin{bmatrix} x \\ y \end{bmatrix}$.  To find the eigenvalues, we solve the equation  $det(A - dI) = 0$. This gives us  $det \begin{bmatrix} 1-d & 0 \\ 0 & 1-d \end{bmatrix} = 0$, which simplifies to $(1-d)(1-d) = 0$. Thus, the eigenvalue is $d = 1$, with $d_1 = d_2 = 1$.

Next, we consider the equation $(A - I)\begin{bmatrix} c_1 \\ c_2 \end{bmatrix} = \begin{bmatrix} 0 \\ 0 \end{bmatrix}$, which expands to $\begin{bmatrix} 0 & 0 \\ 0 & 0 \end{bmatrix} \begin{bmatrix} c_1 \\ c_2 \end{bmatrix} = \begin{bmatrix} 0 \\ 0 \end{bmatrix}$.  Therefore, the above holds true for all vectors $v$ in $\mathbb{R}^2$.  Let us take $v_1 = \begin{bmatrix} 1 \\ 1 \end{bmatrix}$ as a basis for the solutions.  Then, the general solution is given by $X(t) = \lambda e^t \begin{bmatrix} 1 \\ 1 \end{bmatrix}$. 
